Big reorganization of romega/ReflOmegaCore.v: towards a modular and generic romega tactic...
For the moment, nothing is visible yet from the user's point of view 
(hopefully). But internally, we prepare a romega that can works on 
any integer types. ReflOmegaCore is now separated in several modules: 

* First, an interface Int that specifies the minimal amount of things 
  needed on our integer type for romega to work: 
  - int should be a ring (re-use of ring_theory definition ;-)
  - it should come with an total order, compatible with + * -
  - we should have a decidable ternary comparison function
  - moreover, we ask one (and only one!) critical property specific to
    integers:    a<b <-> a<=b-1

* Then a functor IntProperties derives from this interface all the 
  various lemmas on integers that are used in the romega part, 
  in particular the famous OMEGA?? lemmas. 
  
* The romega reflexive part is now in another functor IntOmega, 
  that rely on some Int: no more Z inside. The main changes is
  that Z0 was a constructor whereas our abstract zero isn't. So
  matching Z0 is transformed into (if beq ... 0 then ...). With
  extensive use of && and if then else, it's almost clearer this way.

* Finally, for the moment Z_as_Int show that Z fulfills our interface, 
  and ZOmega = IntOmega(Z_as_Int) is used by the tactic. 


Remains to be done: 
 - revision of the refl_omega to use any Int instead of just Z, 
   and creating a user interface. 
 - Int has no particular reason to use the leibniz equality (only 
   rely on the beq boolean test). Setoids someday ?
 - a version with "semi-ring" for nat ? or rather a generic way to plug 
   additional equations on the fly, e.g. n>=0 for every nat subpart ?




git-svn-id: svn+ssh://scm.gforge.inria.fr/svn/coq/trunk@9966 85f007b7-540e-0410-9357-904b9bb8a0f7

contrib/romega/const_omega.ml
@@ -71,7 +71,7 @@ let coq_modules =
     @ [["Coq"; "omega"; "OmegaLemmas"]]
     @ [["Coq"; "Lists"; "List"]]
     @ [module_refl_path]
-
+    @ [module_refl_path@["ZOmega"]]
 
 let constant = Coqlib.gen_constant_in_modules "Omega" coq_modules
 
@@ -121,8 +121,7 @@ let coq_I = lazy(constant "I")
 let coq_cons =  lazy (constant "cons")
 let coq_nil =  lazy (constant "nil")
 
-let coq_pcons = lazy (constant "Pcons")
-let coq_pnil = lazy (constant "Pnil")
+(* ReflOmegaCore/ZOmega *)
 
 let coq_h_step = lazy (constant "h_step")
 let coq_pair_step = lazy (constant  "pair_step")
@@ -131,7 +130,6 @@ let coq_p_right = lazy (constant  "P_RIGHT")
 let coq_p_invert = lazy (constant  "P_INVERT")
 let coq_p_step = lazy (constant  "P_STEP")
 let coq_p_nop = lazy (constant  "P_NOP")
-
 
 let coq_t_int = lazy (constant  "Tint")
 let coq_t_plus = lazy (constant  "Tplus")
@@ -301,14 +299,7 @@ let mk_list typ l =
 	Term.mkApp (Lazy.force coq_cons, [|typ; step; loop l |]) in
   loop l
 
-let mk_plist l =
-  let rec loop = function
-    | [] ->
-	(Lazy.force coq_pnil)
-    | (step :: l) -> 
-	Term.mkApp (Lazy.force coq_pcons, [| step; loop l |]) in
-  loop l
-
+let mk_plist l = mk_list Term.mkProp l
 
 let mk_shuffle_list l = mk_list (Lazy.force coq_t_fusion) l
 
