contrib/romega/ReflOmegaCore.v
@@ -7,32 +7,852 @@
 
  *************************************************************************)
 
-Require Import Arith.
-Require Import List.
-Require Import Bool.
-Require Import ZArith_base.
-Require Import OmegaLemmas.
+Require Import List Bool Sumbool EqNat Ring_theory Decidable.
+Delimit Scope Int_scope with I.
 
-Open Scope Z_scope.
+(* Abstract Integers. *)
 
-(* \subsection{Definition of basic types} *)
+Module Type Int. 
 
-(* \subsubsection{Environment of propositions (lists) *)
-Inductive PropList : Type :=
-  | Pnil : PropList
-  | Pcons : Prop -> PropList -> PropList.
+  Parameter int : Set. 
 
-(* Access function for the environment with a default *)
-Fixpoint nthProp (n : nat) (l : PropList) (default : Prop) {struct l} :
- Prop :=
-  match n, l with
-  | O, Pcons x l' => x
-  | O, other => default
-  | S m, Pnil => default
-  | S m, Pcons x t => nthProp m t default
-  end.
+  Parameter zero : int. 
+  Parameter one : int. 
+  Parameter plus : int -> int -> int. 
+  Parameter opp : int -> int.
+  Parameter minus : int -> int -> int. 
+  Parameter mult : int -> int -> int.
+
+  Notation "0" := zero : Int_scope.
+  Notation "1" := one : Int_scope. 
+  Infix "+" := plus : Int_scope.
+  Infix "-" := minus : Int_scope.
+  Infix "*" := mult : Int_scope.
+  Notation "- x" := (opp x) : Int_scope.
+
+  Open Scope Int_scope.
+
+  (* First, int is a ring: *)
+  Axiom ring : @ring_theory int 0 1 plus mult minus opp (@eq int).
+
+  (* int should also be ordered: *)
+
+  Parameter le : int -> int -> Prop.
+  Parameter lt : int -> int -> Prop.
+  Parameter ge : int -> int -> Prop.
+  Parameter gt : int -> int -> Prop.
+  Notation "x <= y" := (le x y): Int_scope.
+  Notation "x < y" := (lt x y) : Int_scope.
+  Notation "x >= y" := (ge x y) : Int_scope.
+  Notation "x > y" := (gt x y): Int_scope.
+  Axiom le_lt_iff : forall i j, (i<=j) <-> ~(j<i).
+  Axiom ge_le_iff : forall i j, (i>=j) <-> (j<=i).
+  Axiom gt_lt_iff : forall i j, (i>j) <-> (j<i).
+
+  (* Basic properties of this order *)
+  Axiom lt_trans : forall i j k, i<j -> j<k -> i<k.
+  Axiom lt_not_eq : forall i j, i<j -> i<>j.
+
+  (* Compatibilities *)
+  Axiom lt_0_1 : 0<1.
+  Axiom plus_le_compat : forall i j k l, i<=j -> k<=l -> i+k<=j+l.
+  Axiom opp_le_compat : forall i j, i<=j -> (-j)<=(-i).
+  Axiom mult_lt_compat_l : 
+   forall i j k, 0 < k -> i < j -> k*i<k*j.
+
+  (* We should have a way to decide the equality and the order*)  
+  Parameter compare : int -> int -> comparison.
+  Infix "?=" := compare (at level 70, no associativity) : Int_scope.
+  Axiom compare_Eq : forall i j, compare i j = Eq <-> i=j.
+  Axiom compare_Lt : forall i j, compare i j = Lt <-> i<j.
+  Axiom compare_Gt : forall i j, compare i j = Gt <-> i>j.
+
+  (* Up to here, these requirements could be fulfilled 
+     by any totally ordered ring. Let's now be int-specific: *)
+  Axiom le_lt_int : forall x y, x<y <-> x<=y+-(1).
+
+  (* Btw, lt_0_1 could be deduced from this last axiom *)
+
+End Int.
+
+
+
+(* Of course, Z is a model for our abstract int *)
+
+Module Z_as_Int <: Int.
+
+  Require Import ZArith_base.
+  Open Scope Z_scope.
+
+  Definition int := Z. 
+  Definition zero := 0. 
+  Definition one := 1. 
+  Definition plus := Zplus.
+  Definition opp := Zopp.
+  Definition minus := Zminus.
+  Definition mult := Zmult.
+
+  Lemma ring : @ring_theory int zero one plus mult minus opp (@eq int).
+  Proof.
+  constructor.
+  exact Zplus_0_l.
+  exact Zplus_comm.
+  exact Zplus_assoc.
+  exact Zmult_1_l.
+  exact Zmult_comm.
+  exact Zmult_assoc.
+  exact Zmult_plus_distr_l.
+  unfold minus, Zminus; auto.
+  exact Zplus_opp_r.
+  Qed.
+
+  Definition le := Zle.
+  Definition lt := Zlt.
+  Definition ge := Zge.
+  Definition gt := Zgt.
+  Lemma le_lt_iff : forall i j, (i<=j) <-> ~(j<i).
+  Proof.
+   split; intros.
+   apply Zle_not_lt; auto.
+   rewrite <- Zge_iff_le.
+   apply Znot_lt_ge; auto.
+  Qed.
+  Definition ge_le_iff := Zge_iff_le.
+  Definition gt_lt_iff := Zgt_iff_lt.
+
+  Definition lt_trans := Zlt_trans.
+  Definition lt_not_eq := Zlt_not_eq.
+
+  Definition lt_0_1 := Zlt_0_1.
+  Definition plus_le_compat := Zplus_le_compat.
+  Definition mult_lt_compat_l := Zmult_lt_compat_l.
+  Lemma opp_le_compat : forall i j, i<=j -> (-j)<=(-i).
+  Proof.
+  unfold Zle; intros; rewrite <- Zcompare_opp; auto.
+  Qed.
+
+  Definition compare := Zcompare.
+  Definition compare_Eq := Zcompare_Eq_iff_eq.
+  Lemma compare_Lt : forall i j, compare i j = Lt <-> i<j.
+  Proof. intros; unfold compare, Zlt; intuition. Qed.
+  Lemma compare_Gt : forall i j, compare i j = Gt <-> i>j.
+  Proof. intros; unfold compare, Zgt; intuition. Qed.
+
+  Lemma le_lt_int : forall x y, x<y <-> x<=y+-(1).
+  Proof.
+   intros; split; intros.
+   generalize (Zlt_left _ _ H); simpl; intros.
+   apply Zle_left_rev; auto.
+   apply Zlt_0_minus_lt.
+   generalize (Zplus_le_lt_compat x (y+-1) (-x) (-x+1) H).
+   rewrite Zplus_opp_r.
+   rewrite <-Zplus_assoc.
+   rewrite (Zplus_permute (-1)).
+   simpl in *.
+   rewrite Zplus_0_r.
+   intro H'; apply H'.
+   replace (-x+1) with (Zsucc (-x)); auto.
+   apply Zlt_succ.
+  Qed.
+
+End Z_as_Int.  
+
+
+
+
+Module IntProperties (I:Int). 
+ Import I.
+ 
+ (* Primo, some consequences of being a ring theory... *)
+ 
+ Definition two := 1+1.
+ Notation "2" := two : Int_scope. 
+
+ (* Aliases for properties packed in the ring record. *)
+
+ Definition plus_assoc := ring.(Radd_assoc).
+ Definition plus_comm := ring.(Radd_comm).
+ Definition plus_0_l := ring.(Radd_0_l).
+ Definition mult_assoc := ring.(Rmul_assoc). 
+ Definition mult_comm := ring.(Rmul_comm).
+ Definition mult_1_l := ring.(Rmul_1_l).
+ Definition mult_plus_distr_r := ring.(Rdistr_l).
+ Definition opp_def := ring.(Ropp_def).
+ Definition minus_def := ring.(Rsub_def).
+
+ Opaque plus_assoc plus_comm plus_0_l mult_assoc mult_comm mult_1_l 
+  mult_plus_distr_r opp_def minus_def.
+
+ (* More facts about plus *)
+
+ Lemma plus_0_r : forall x, x+0 = x.
+ Proof. intros; rewrite plus_comm; apply plus_0_l. Qed.
+
+ Lemma plus_0_r_reverse : forall x, x = x+0.
+ Proof. intros; symmetry; apply plus_0_r. Qed. 
+
+ Lemma plus_assoc_reverse : forall x y z, x+y+z = x+(y+z).
+ Proof. intros; symmetry; apply plus_assoc. Qed.
+
+ Lemma plus_permute : forall x y z, x+(y+z) = y+(x+z).
+ Proof. intros; do 2 rewrite plus_assoc; f_equal; apply plus_comm. Qed.
+
+ Lemma plus_reg_l : forall x y z, x+y = x+z -> y = z.
+ Proof. 
+  intros.
+  rewrite (plus_0_r_reverse y), (plus_0_r_reverse z), <-(opp_def x).
+  now rewrite plus_permute, plus_assoc, H, <- plus_assoc, plus_permute. 
+ Qed.
+
+ (* More facts about mult *) 
    
-(* \subsubsection{Définition of reified integer expressions}
+ Lemma mult_assoc_reverse : forall x y z, x*y*z = x*(y*z).
+ Proof. intros; symmetry; apply mult_assoc. Qed.
+
+ Lemma mult_plus_distr_l : forall x y z, x*(y+z)=x*y+x*z.
+ Proof.
+  intros.
+  rewrite (mult_comm x (y+z)), (mult_comm x y), (mult_comm x z).
+  apply mult_plus_distr_r.
+ Qed.
+
+ Lemma mult_0_l : forall x, 0*x = 0.
+ Proof. 
+  intros.
+  generalize (mult_plus_distr_r 0 1 x).
+  rewrite plus_0_l, mult_1_l, plus_comm; intros.
+  apply plus_reg_l with x.
+  rewrite <- H.
+  apply plus_0_r_reverse.
+ Qed.
+ 
+
+ (* More facts about opp *)
+
+ Definition plus_opp_r := opp_def.
+
+ Lemma plus_opp_l : forall x, -x + x = 0.
+ Proof. intros; now rewrite plus_comm, opp_def. Qed.
+
+ Lemma mult_opp_comm : forall x y, - x * y = x * - y.
+ Proof.
+  intros.
+  apply plus_reg_l with (x*y).
+  rewrite <- mult_plus_distr_l, <- mult_plus_distr_r.
+  now rewrite opp_def, opp_def, mult_0_l, mult_comm, mult_0_l.
+ Qed.
+
+ Lemma opp_eq_mult_neg_1 : forall x, -x = x * -(1).
+ Proof.
+  intros; now rewrite mult_comm, mult_opp_comm, mult_1_l.
+ Qed.
+
+ Lemma opp_involutive : forall x, -(-x) = x.
+ Proof.
+  intros.
+  apply plus_reg_l with (-x).
+  now rewrite opp_def, plus_comm, opp_def.
+ Qed.
+
+ Lemma opp_plus_distr : forall x y, -(x+y) = -x + -y.
+ Proof.
+  intros.
+  apply plus_reg_l with (x+y).
+  rewrite opp_def.
+  rewrite plus_permute.
+  do 2 rewrite plus_assoc.
+  now rewrite (plus_comm (-x)), opp_def, plus_0_l, opp_def.
+ Qed.
+
+ Lemma opp_mult_distr_r : forall x y, -(x*y) = x * -y.
+ Proof.
+  intros.
+  rewrite <- mult_opp_comm.
+  apply plus_reg_l with (x*y).
+  now rewrite opp_def, <-mult_plus_distr_r, opp_def, mult_0_l.
+ Qed.  
+
+ Lemma egal_left : forall n m, n=m -> n+-m = 0.
+ Proof. intros; subst; apply opp_def. Qed.
+
+ Lemma ne_left_2 : forall x y : int, x<>y -> 0<>(x + - y).
+ Proof.
+ intros; swap H.
+ apply (plus_reg_l (-y)).
+ now rewrite plus_opp_l, plus_comm, H0.
+ Qed.
+
+ (* Special lemmas for factorisation. *)
+
+ Lemma red_factor0 : forall n, n = n*1.
+ Proof. symmetry; rewrite mult_comm; apply mult_1_l. Qed.
+
+ Lemma red_factor1 : forall n, n+n = n*2.
+ Proof. 
+  intros; unfold two.
+  now rewrite mult_comm, mult_plus_distr_r, mult_1_l.
+ Qed.
+
+ Lemma red_factor2 : forall n m, n + n*m = n * (1+m).
+ Proof.
+  intros; rewrite mult_plus_distr_l.
+  f_equal; now rewrite mult_comm, mult_1_l.
+ Qed.
+
+ Lemma red_factor3 : forall n m, n*m + n = n*(1+m).
+ Proof. intros; now rewrite plus_comm, red_factor2. Qed.
+
+ Lemma red_factor4 : forall n m p, n*m + n*p = n*(m+p).
+ Proof. 
+  intros; now rewrite mult_plus_distr_l.
+ Qed.
+ 
+ Lemma red_factor5 : forall n m , n * 0 + m = m.
+ Proof. intros; now rewrite mult_comm, mult_0_l, plus_0_l. Qed.
+
+ Definition red_factor6 := plus_0_r_reverse.
+
+
+ (* Specialized distributivities *)
+
+ Hint Rewrite mult_plus_distr_l mult_plus_distr_r mult_assoc : int.
+ Hint Rewrite <- plus_assoc : int.
+
+ Lemma OMEGA10 :
+  forall v c1 c2 l1 l2 k1 k2 : int,
+  (v * c1 + l1) * k1 + (v * c2 + l2) * k2 =
+  v * (c1 * k1 + c2 * k2) + (l1 * k1 + l2 * k2).
+ Proof.
+  intros; autorewrite with int; f_equal; now rewrite plus_permute.
+ Qed.
+
+ Lemma OMEGA11 :
+  forall v1 c1 l1 l2 k1 : int,
+  (v1 * c1 + l1) * k1 + l2 = v1 * (c1 * k1) + (l1 * k1 + l2).
+ Proof.
+  intros; now autorewrite with int.
+ Qed.
+
+ Lemma OMEGA12 :
+  forall v2 c2 l1 l2 k2 : int,
+  l1 + (v2 * c2 + l2) * k2 = v2 * (c2 * k2) + (l1 + l2 * k2).
+ Proof.
+  intros; autorewrite with int; now rewrite plus_permute.
+ Qed.
+
+ Lemma OMEGA13 :
+  forall v l1 l2 x : int,
+  v * -x + l1 + (v * x + l2) = l1 + l2.
+ Proof.
+ intros; autorewrite with int.
+ rewrite plus_permute; f_equal.
+ rewrite plus_assoc.
+ now rewrite <- mult_plus_distr_l, plus_opp_l, mult_comm, mult_0_l, plus_0_l.
+ Qed.
+
+ Lemma OMEGA15 :
+  forall v c1 c2 l1 l2 k2 : int,
+  v * c1 + l1 + (v * c2 + l2) * k2 = v * (c1 + c2 * k2) + (l1 + l2 * k2).
+ Proof.
+  intros; autorewrite with int; f_equal; now rewrite plus_permute.
+ Qed.
+
+ Lemma OMEGA16 : forall v c l k : int, (v * c + l) * k = v * (c * k) + l * k.
+ Proof.
+  intros; now autorewrite with int.
+ Qed.
+
+ Lemma sum1 : forall a b c d : int, 0 = a -> 0 = b -> 0 = a * c + b * d.
+ Proof.
+ intros; elim H; elim H0; simpl in |- *; auto.
+ now rewrite mult_0_l, mult_0_l, plus_0_l.
+ Qed.
+
+
+ (* Secondo, some results about order (and equality) *)  
+
+ Lemma lt_irrefl : forall n, ~ n<n.
+ Proof.
+ intros n H.
+ elim (lt_not_eq _ _ H); auto.
+ Qed.
+
+ Lemma lt_antisym : forall n m, n<m -> m<n -> False.
+ Proof.
+ intros; elim (lt_irrefl _ (lt_trans _ _ _ H H0)); auto.
+ Qed.
+
+ Lemma lt_le_weak : forall n m, n<m -> n<=m.
+ Proof.
+  intros; rewrite le_lt_iff; intro H'; eapply lt_antisym; eauto.
+ Qed.
+
+ Lemma le_refl : forall n, n<=n.
+ Proof.
+ intros; rewrite le_lt_iff; apply lt_irrefl; auto.
+ Qed.
+
+ Lemma le_antisym : forall n m, n<=m -> m<=n -> n=m.
+ Proof.
+ intros n m; do 2 rewrite le_lt_iff; intros.
+ rewrite <- compare_Lt in H0.
+ rewrite <- gt_lt_iff, <- compare_Gt in H.
+ rewrite <- compare_Eq.
+ destruct compare; intuition.
+ Qed.
+
+ Lemma lt_eq_lt_dec : forall n m, { n<m }+{ n=m }+{ m<n }.
+ Proof.
+  intros.
+  generalize (compare_Lt n m)(compare_Eq n m)(compare_Gt n m).
+  destruct compare; [ left; right | left; left | right ]; intuition.
+  rewrite gt_lt_iff in H1; intuition.
+ Qed.
+
+ Lemma lt_dec : forall n m: int, { n<m } + { ~n<m }.
+ Proof.
+  intros.
+  generalize (compare_Lt n m)(compare_Eq n m)(compare_Gt n m).
+  destruct compare; [ right | left | right ]; intuition discriminate.
+ Qed.
+
+ Lemma lt_le_iff : forall n m, (n<m) <-> ~(m<=n).
+ Proof.
+  intros.
+  rewrite le_lt_iff.
+  destruct (lt_dec n m); intuition.
+ Qed.
+
+ Lemma le_dec : forall n m: int, { n<=m } + { ~n<=m }.
+ Proof.
+  intros; destruct (lt_dec m n); [right|left]; rewrite le_lt_iff; intuition.
+ Qed.
+
+ Lemma le_lt_dec : forall n m, { n<=m } + { m<n }.
+ Proof.
+  intros; destruct (le_dec n m); [left|right]; auto; now rewrite lt_le_iff.
+ Qed.
+
+
+ Definition beq i j := match compare i j with Eq => true | _ => false end.
+
+ Lemma beq_iff : forall i j, beq i j = true <-> i=j.
+ Proof.
+ intros; unfold beq; generalize (compare_Eq i j).
+ destruct compare; intuition discriminate.
+ Qed.
+                               
+ Lemma beq_true : forall i j, beq i j = true -> i=j.
+ Proof.
+ intros.
+ rewrite <- beq_iff; auto.
+ Qed.
+
+ Lemma beq_false : forall i j, beq i j = false -> i<>j.
+ Proof.
+ intros.
+ intro H'.
+ rewrite <- beq_iff in H'; rewrite H' in H; discriminate.
+ Qed.
+
+ Lemma eq_dec : forall n m:int, { n=m } + { n<>m }.
+ Proof.
+  intros; generalize (beq_iff n m); destruct beq; [left|right]; intuition.
+ Qed.
+
+ Definition bgt i j := match compare i j with Gt => true | _ => false end.
+
+ Lemma bgt_iff : forall i j, bgt i j = true <-> i>j.
+ Proof.
+ intros; unfold bgt; generalize (compare_Gt i j).
+ destruct compare; intuition discriminate.
+ Qed.
+
+ Lemma bgt_true : forall i j, bgt i j = true -> i>j.
+ Proof. intros; now rewrite <- bgt_iff. Qed.
+
+ Lemma bgt_false : forall i j, bgt i j = false -> i<=j.
+ Proof. 
+  intros.
+  rewrite le_lt_iff, <-gt_lt_iff, <-bgt_iff; intro H'; now rewrite H' in H.
+ Qed.
+
+ Lemma le_is_lt_or_eq : forall n m, n<=m -> { n<m } + { n=m }.
+ Proof.
+  intros.
+  destruct (eq_dec n m) as [H'|H'].
+  right; intuition.
+  left; rewrite lt_le_iff.
+  swap H'.
+  apply le_antisym; auto.
+ Qed.
+
+ Lemma le_neq_lt : forall n m, n<=m -> n<>m -> n<m.
+ Proof.
+  intros.
+  destruct (le_is_lt_or_eq _ _ H); intuition.
+ Qed.
+
+ Lemma le_trans : forall n m p, n<=m -> m<=p -> n<=p.
+ Proof.
+  intros n m p; do 3 rewrite le_lt_iff; intros A B C.
+  destruct (lt_eq_lt_dec p m) as [[H|H]|H]; subst; auto.
+  generalize (lt_trans _ _ _ H C); intuition.
+ Qed.
+ 
+ (* order and operations *)
+
+ Lemma le_0_neg : forall n, 0 <= n <-> -n <= 0.
+ Proof.
+ intros.
+ pattern 0 at 2; rewrite <- (mult_0_l (-(1))).
+ rewrite <- opp_eq_mult_neg_1.
+ split; intros.
+ apply opp_le_compat; auto.
+ rewrite <-(opp_involutive 0), <-(opp_involutive n).
+ apply opp_le_compat; auto.
+ Qed.
+
+ Lemma le_0_neg' : forall n, n <= 0 <-> 0 <= -n.
+ Proof.
+ intros; rewrite le_0_neg, opp_involutive; intuition.
+ Qed.
+
+ Lemma plus_le_reg_r : forall n m p, n + p <= m + p -> n <= m.
+ Proof.
+ intros.
+ replace n with ((n+p)+-p).
+ replace m with ((m+p)+-p).
+ apply plus_le_compat; auto.
+ apply le_refl.
+ now rewrite <- plus_assoc, opp_def, plus_0_r.
+ now rewrite <- plus_assoc, opp_def, plus_0_r.
+ Qed.
+
+ Lemma plus_le_lt_compat : forall n m p q, n<=m -> p<q -> n+p<m+q.
+ Proof.
+ intros.
+ apply le_neq_lt.
+ apply plus_le_compat; auto.
+ apply lt_le_weak; auto.
+ rewrite lt_le_iff in H0.
+ swap H0.
+ apply plus_le_reg_r with m.
+ rewrite (plus_comm q m), <-H1, (plus_comm p m).
+ apply plus_le_compat; auto.
+ apply le_refl; auto.
+ Qed.
+
+ Lemma plus_lt_compat : forall n m p q, n<m -> p<q -> n+p<m+q.
+ Proof.
+ intros.
+ apply plus_le_lt_compat; auto.
+ apply lt_le_weak; auto.
+ Qed.
+
+ Lemma opp_lt_compat : forall n m, n<m -> -m < -n.
+ Proof.
+ intros n m; do 2 rewrite lt_le_iff; intros H; swap H.
+ rewrite <-(opp_involutive m), <-(opp_involutive n).
+ apply opp_le_compat; auto.
+ Qed.
+
+ Lemma lt_0_neg : forall n, 0 < n <-> -n < 0.
+ Proof.
+ intros.
+ pattern 0 at 2; rewrite <- (mult_0_l (-(1))).
+ rewrite <- opp_eq_mult_neg_1.
+ split; intros.
+ apply opp_lt_compat; auto.
+ rewrite <-(opp_involutive 0), <-(opp_involutive n).
+ apply opp_lt_compat; auto.
+ Qed.
+
+ Lemma lt_0_neg' : forall n, n < 0 <-> 0 < -n.
+ Proof.
+ intros; rewrite lt_0_neg, opp_involutive; intuition.
+ Qed.
+
+ Lemma mult_lt_0_compat : forall n m, 0 < n -> 0 < m -> 0 < n*m.
+ Proof.
+ intros.
+ rewrite <- (mult_0_l n), mult_comm.
+ apply mult_lt_compat_l; auto.
+ Qed.
+
+ Lemma mult_integral : forall n m, n * m = 0 -> n = 0 \/ m = 0.
+ Proof.
+ intros.
+ destruct (lt_eq_lt_dec n 0) as [[Hn|Hn]|Hn]; auto; 
+  destruct (lt_eq_lt_dec m 0) as [[Hm|Hm]|Hm]; auto; elimtype False.
+
+ rewrite lt_0_neg' in Hn.
+ rewrite lt_0_neg' in Hm.
+ generalize (mult_lt_0_compat _ _ Hn Hm).
+ rewrite <- opp_mult_distr_r, mult_comm, <- opp_mult_distr_r, opp_involutive.
+ rewrite mult_comm, H.
+ exact (lt_irrefl 0).
+
+ rewrite lt_0_neg' in Hn.
+ generalize (mult_lt_0_compat _ _ Hn Hm).
+ rewrite mult_comm, <- opp_mult_distr_r, mult_comm.
+ rewrite H.
+ rewrite opp_eq_mult_neg_1, mult_0_l.
+ exact (lt_irrefl 0).
+
+ rewrite lt_0_neg' in Hm.
+ generalize (mult_lt_0_compat _ _ Hn Hm).
+ rewrite <- opp_mult_distr_r.
+ rewrite H.
+ rewrite opp_eq_mult_neg_1, mult_0_l.
+ exact (lt_irrefl 0).
+
+ generalize (mult_lt_0_compat _ _ Hn Hm).
+ rewrite H.
+ exact (lt_irrefl 0).
+ Qed.
+
+ Lemma mult_le_compat : 
+   forall i j k l, i<=j -> k<=l -> 0<=i -> 0<=k -> i*k<=j*l.
+ Proof.
+ intros.
+ destruct (le_is_lt_or_eq _ _ H1).
+
+ apply le_trans with (i*l).
+ destruct (le_is_lt_or_eq _ _ H0); [ | subst; apply le_refl].
+ apply lt_le_weak.
+ apply mult_lt_compat_l; auto.
+
+ generalize (le_trans _ _ _ H2 H0); clear H0 H1 H2; intros.
+ rewrite (mult_comm i), (mult_comm j).
+ destruct (le_is_lt_or_eq _ _ H0); 
+  [ | subst; do 2 rewrite mult_0_l; apply le_refl].
+ destruct (le_is_lt_or_eq _ _ H); 
+  [ | subst; apply le_refl].
+ apply lt_le_weak.
+ apply mult_lt_compat_l; auto.
+
+ subst i.
+ rewrite mult_0_l.
+ generalize (le_trans _ _ _ H2 H0); clear H0 H1 H2; intros.
+ destruct (le_is_lt_or_eq _ _ H); 
+  [ | subst; rewrite mult_0_l; apply le_refl].
+ destruct (le_is_lt_or_eq _ _ H0); 
+  [ | subst; rewrite mult_comm, mult_0_l; apply le_refl].
+ apply lt_le_weak.
+ apply mult_lt_0_compat; auto.
+ Qed.
+
+ Lemma sum5 :
+ forall a b c d : int, c <> 0 -> 0 <> a -> 0 = b -> 0 <> a * c + b * d.
+ Proof.
+ intros.
+ subst b; rewrite mult_0_l, plus_0_r.
+ swap H.
+ symmetry in H1; destruct (mult_integral _ _ H1); congruence.
+ Qed.
+
+ Lemma one_neq_zero : 1 <> 0.
+ Proof.
+ red; intro.
+ symmetry in H.
+ apply (lt_not_eq 0 1); auto.
+ apply lt_0_1.
+ Qed.
+
+ Lemma minus_one_neq_zero : -(1) <> 0.
+ Proof.
+ apply lt_not_eq.
+ rewrite <- lt_0_neg.
+ apply lt_0_1.
+ Qed.
+
+ Lemma le_left : forall n m, n <= m -> 0 <= m + - n.
+ Proof.
+  intros.
+  rewrite <- (opp_def m).
+  apply plus_le_compat.
+  apply le_refl.
+  apply opp_le_compat; auto.
+ Qed.
+
+ Lemma OMEGA2 : forall x y, 0 <= x -> 0 <= y -> 0 <= x + y.
+ Proof.
+ intros.
+ replace 0 with (0+0).
+ apply plus_le_compat; auto.
+ rewrite plus_0_l; auto.
+ Qed.
+
+ Lemma OMEGA8 : forall x y, 0 <= x -> 0 <= y -> x = - y -> x = 0.
+ Proof.
+ intros.
+ assert (y=-x).
+  subst x; symmetry; apply opp_involutive.
+ clear H1; subst y.
+ destruct (eq_dec 0 x) as [H'|H']; auto.
+ assert (H'':=le_neq_lt _ _ H H').
+ generalize (plus_le_lt_compat _ _ _ _ H0 H'').
+ rewrite plus_opp_l, plus_0_l.
+ intros.
+ elim (lt_not_eq _ _ H1); auto.
+ Qed.
+
+ Lemma sum2 :
+ forall a b c d : int, 0 <= d -> 0 = a -> 0 <= b -> 0 <= a * c + b * d.
+ Proof.
+ intros.
+ subst a; rewrite mult_0_l, plus_0_l.
+ rewrite <- (mult_0_l 0).
+ apply mult_le_compat; auto; apply le_refl.
+ Qed.
+
+ Lemma sum3 :
+ forall a b c d : int,
+  0 <= c -> 0 <= d -> 0 <= a -> 0 <= b -> 0 <= a * c + b * d.
+ Proof.
+ intros.
+ rewrite <- (plus_0_l 0).
+ apply plus_le_compat; auto.
+ rewrite <- (mult_0_l 0).
+ apply mult_le_compat; auto; apply le_refl.
+ rewrite <- (mult_0_l 0).
+ apply mult_le_compat; auto; apply le_refl.
+ Qed.
+
+ Lemma sum4 : forall k : int, k>0 -> 0 <= k.
+ Proof.
+ intros k; rewrite gt_lt_iff; apply lt_le_weak.
+ Qed.
+
+ (* Lemmas specific to integers (they use lt_le_int) *)
+
+ Lemma lt_left : forall n m, n < m -> 0 <= m + -(1) + - n.
+ Proof.
+ intros; apply le_left.
+ now rewrite <- le_lt_int.
+ Qed.
+
+ Lemma lt_left_inv : forall x y, 0 <= y + -(1) + - x -> x < y.
+ Proof.
+ intros.
+ generalize (plus_le_compat _ _ _ _ H (le_refl x)); clear H.
+ now rewrite plus_0_l, <-plus_assoc, plus_opp_l, plus_0_r, le_lt_int.
+ Qed.
+
+ Lemma OMEGA4 : forall x y z, x > 0 -> y > x -> z * y + x <> 0.
+ Proof.
+ intros.
+ intro H'.
+ rewrite gt_lt_iff in H,H0.
+ destruct (lt_eq_lt_dec z 0) as [[G|G]|G].
+
+ rewrite lt_0_neg' in G.
+ generalize (plus_le_lt_compat _ _ _ _ (le_refl (z*y)) H0).
+ rewrite H'.
+ pattern y at 2; rewrite <-(mult_1_l y), <-mult_plus_distr_r.
+ intros.
+ rewrite le_lt_int in G.
+ rewrite <- opp_plus_distr in G.
+ assert (0 < y) by (apply lt_trans with x; auto).
+ generalize (mult_le_compat _ _ _ _ G (lt_le_weak _ _ H2) (le_refl 0) (le_refl 0)).
+ rewrite mult_0_l, mult_comm, <- opp_mult_distr_r, mult_comm, <-le_0_neg', le_lt_iff.
+ intuition.
+
+ subst; rewrite mult_0_l, plus_0_l in H'; subst.
+ apply (lt_not_eq _ _ H); auto.
+
+ apply (lt_not_eq 0 (z*y+x)); auto.
+ rewrite <- (plus_0_l 0).
+ apply plus_lt_compat; auto.
+ apply mult_lt_0_compat; auto.
+ apply lt_trans with x; auto.
+ Qed. 
+
+ Lemma OMEGA19 : forall x, x<>0 -> 0 <= x + -(1) \/ 0 <= x * -(1) + -(1).
+ Proof.
+ intros.
+ do 2 rewrite <- le_lt_int.
+ rewrite <- opp_eq_mult_neg_1.
+ destruct (lt_eq_lt_dec 0 x) as [[H'|H']|H'].
+ auto.
+ congruence.
+ right.
+ rewrite <-(mult_0_l (-(1))), <-(opp_eq_mult_neg_1 0).
+ apply opp_lt_compat; auto.
+ Qed.
+
+ Lemma mult_le_approx : 
+  forall n m p, n > 0 -> n > p -> 0 <= m * n + p -> 0 <= m.
+ Proof.
+ intros n m p.
+ do 2 rewrite gt_lt_iff.
+ do 2 rewrite le_lt_iff; intros.
+ swap H1.
+ rewrite lt_0_neg' in H2.
+ rewrite lt_0_neg'.
+ rewrite opp_plus_distr.
+ rewrite mult_comm, opp_mult_distr_r.
+ rewrite le_lt_int.
+ rewrite <- plus_assoc, (plus_comm (-p)), plus_assoc.
+ apply lt_left.
+ rewrite le_lt_int.
+ rewrite le_lt_int in H0.
+ apply le_trans with (n+-(1)); auto.
+ apply plus_le_compat; [ | apply le_refl ].
+ rewrite le_lt_int in H2.
+ generalize (mult_le_compat _ _ _ _ (lt_le_weak _ _ H) H2 (le_refl 0) (le_refl 0)).
+ rewrite mult_0_l.
+ rewrite mult_plus_distr_l.
+ rewrite <- opp_eq_mult_neg_1.
+ intros.
+ generalize (plus_le_compat _ _ _ _ (le_refl n) H1).
+ now rewrite plus_permute, opp_def, plus_0_r, plus_0_r.
+ Qed.
+
+ (* Some decidabilities *)
+
+ Lemma dec_eq : forall i j:int, decidable (i=j).
+ Proof.
+  red; intros; destruct (eq_dec i j); auto.
+ Qed.
+
+ Lemma dec_ne : forall i j:int, decidable (i<>j).
+ Proof.
+  red; intros; destruct (eq_dec i j); auto.
+ Qed.
+
+ Lemma dec_le : forall i j:int, decidable (i<=j).
+ Proof.
+  red; intros; destruct (le_dec i j); auto.
+ Qed.
+
+ Lemma dec_lt : forall i j:int, decidable (i<j).
+ Proof.
+  red; intros; destruct (lt_dec i j); auto.
+ Qed.
+
+ Lemma dec_ge : forall i j:int, decidable (i>=j).
+ Proof.
+  red; intros; rewrite ge_le_iff; destruct (le_dec j i); auto.
+ Qed.
+
+ Lemma dec_gt : forall i j:int, decidable (i>j).
+ Proof.
+  red; intros; rewrite gt_lt_iff; destruct (lt_dec j i); auto.
+ Qed.
+
+End IntProperties.
+
+
+
+
+Module IntOmega (I:Int).
+Import I.
+Module IP:=IntProperties(I).
+Import IP.
+   
+(* \subsubsection{Definition of reified integer expressions}
    Terms are either:
    \begin{itemize}
    \item integers [Tint]
@@ -41,7 +861,7 @@ Fixpoint nthProp (n : nat) (l : PropList) (default : Prop) {struct l} :
    The last two are translated in additions and products. *)
 
 Inductive term : Set :=
-  | Tint : Z -> term
+  | Tint : int -> term
   | Tplus : term -> term -> term
   | Tmult : term -> term -> term
   | Tminus : term -> term -> term
@@ -49,6 +869,7 @@ Inductive term : Set :=
   | Tvar : nat -> term.
 
 Delimit Scope romega_scope with term.
+Arguments Scope Tint [Int_scope].
 Arguments Scope Tplus [romega_scope romega_scope].
 Arguments Scope Tmult [romega_scope romega_scope].
 Arguments Scope Tminus [romega_scope romega_scope].
@@ -61,17 +882,18 @@ Notation "- x" := (Topp x) : romega_scope.
 Notation "[ x ]" := (Tvar x) (at level 1) : romega_scope.
 
 (* \subsubsection{Definition of reified goals} *)
+
 (* Very restricted definition of handled predicates that should be extended
    to cover a wider set of operations.
    Taking care of negations and disequations require solving more than a
    goal in parallel. This is a major improvement over previous versions. *)
 
 Inductive proposition : Set :=
-  | EqTerm : term -> term -> proposition (* egalité entre termes *)
-  | LeqTerm : term -> term -> proposition (* plus petit ou egal *)
-  | TrueTerm : proposition (* vrai *)
-  | FalseTerm : proposition (* faux *)
-  | Tnot : proposition -> proposition (* négation *)
+  | EqTerm : term -> term -> proposition (* equality between terms *)
+  | LeqTerm : term -> term -> proposition (* less or equal on terms *)
+  | TrueTerm : proposition (* true *)
+  | FalseTerm : proposition (* false *)
+  | Tnot : proposition -> proposition (* negation *)
   | GeqTerm : term -> term -> proposition
   | GtTerm : term -> term -> proposition
   | LtTerm : term -> term -> proposition
@@ -87,7 +909,7 @@ Notation hyps := (list proposition).
 (* Definition of lists of subgoals  (set of open goals) *)
 Notation lhyps := (list hyps).
 
-(* a syngle goal packed in a subgoal list *)
+(* a single goal packed in a subgoal list *)
 Notation singleton := (fun a : hyps => a :: nil).
 
 (* an absurd goal *)
@@ -110,24 +932,22 @@ Inductive t_fusion : Set :=
 
 (* \subsubsection{Rewriting steps to normalize terms} *)
 Inductive step : Set := 
- (* apply the rewriting steps to both subterms of an operation *)
-  | C_DO_BOTH :
-      step -> step -> step
-              (* apply the rewriting step to the first branch *)
+  (* apply the rewriting steps to both subterms of an operation *)
+  | C_DO_BOTH : step -> step -> step
+  (* apply the rewriting step to the first branch *)
   | C_LEFT : step -> step
-             (* apply the rewriting step to the second branch *)
+  (* apply the rewriting step to the second branch *)
   | C_RIGHT : step -> step
-              (* apply two steps consecutively to a term *)
-  | C_SEQ : step -> step -> step
-                    (* empty step *)
-  | C_NOP : step
-      (* the following operations correspond to actual rewriting *)
+  (* apply two steps consecutively to a term *)
+  | C_SEQ : step -> step -> step 
+  (* empty step *)
+  | C_NOP : step 
+  (* the following operations correspond to actual rewriting *)
   | C_OPP_PLUS : step
   | C_OPP_OPP : step
   | C_OPP_MULT_R : step
-  | C_OPP_ONE :
-      step
-      (* This is a special step that reduces the term (computation) *)
+  | C_OPP_ONE : step
+  (* This is a special step that reduces the term (computation) *)
   | C_REDUCE : step
   | C_MULT_PLUS_DISTR : step
   | C_MULT_OPP_LEFT : step
@@ -152,261 +972,98 @@ Inductive step : Set :=
    the trace coming from the decision procedure Omega. *)
 
 Inductive t_omega : Set :=
- (* n = 0 n!= 0 *)
+  (* n = 0 and n!= 0 *)
   | O_CONSTANT_NOT_NUL : nat -> t_omega
-  | O_CONSTANT_NEG :
-      nat -> t_omega
-      (* division et approximation of an equation *)
-  | O_DIV_APPROX :
-      Z ->
-      Z ->
-      term ->
-      nat ->
-      t_omega -> nat -> t_omega
-                 (* no solution because no exact division *)
-  | O_NOT_EXACT_DIVIDE :
-      Z -> Z -> term -> nat -> nat -> t_omega
-                               (* exact division *)
-  | O_EXACT_DIVIDE : Z -> term -> nat -> t_omega -> nat -> t_omega
-  | O_SUM : Z -> nat -> Z -> nat -> list t_fusion -> t_omega -> t_omega
+  | O_CONSTANT_NEG : nat -> t_omega
+  (* division and approximation of an equation *)
+  | O_DIV_APPROX : int -> int -> term -> nat -> t_omega -> nat -> t_omega
+  (* no solution because no exact division *)
+  | O_NOT_EXACT_DIVIDE : int -> int -> term -> nat -> nat -> t_omega
+  (* exact division *)
+  | O_EXACT_DIVIDE : int -> term -> nat -> t_omega -> nat -> t_omega
+  | O_SUM : int -> nat -> int -> nat -> list t_fusion -> t_omega -> t_omega
   | O_CONTRADICTION : nat -> nat -> nat -> t_omega
   | O_MERGE_EQ : nat -> nat -> nat -> t_omega -> t_omega
   | O_SPLIT_INEQ : nat -> nat -> t_omega -> t_omega -> t_omega
   | O_CONSTANT_NUL : nat -> t_omega
   | O_NEGATE_CONTRADICT : nat -> nat -> t_omega
   | O_NEGATE_CONTRADICT_INV : nat -> nat -> nat -> t_omega
-  | O_STATE : Z -> step -> nat -> nat -> t_omega -> t_omega.
+  | O_STATE : int -> step -> nat -> nat -> t_omega -> t_omega.
 
-(* \subsubsection{Règles pour normaliser les hypothèses} *)
-(* Ces règles indiquent comment normaliser les propositions utiles 
-   de chaque hypothèse utile avant la décomposition des hypothèses et 
-   incluent l'étape d'inversion pour la suppression des négations *)
+(* \subsubsection{Rules for normalizing the hypothesis} *)
+(* These rules indicate how to normalize useful propositions 
+   of each useful hypothesis before the decomposition of hypothesis. 
+   The rules include the inversion phase for negation removal. *)
+
 Inductive p_step : Set :=
   | P_LEFT : p_step -> p_step
   | P_RIGHT : p_step -> p_step
   | P_INVERT : step -> p_step
   | P_STEP : step -> p_step
   | P_NOP : p_step.
-(* Liste des normalisations a effectuer : avec un constructeur dans le
-   type [p_step] permettant
-   de parcourir à la fois les branches gauches et droit, on pourrait n'avoir
-   qu'une normalisation par hypothèse. Et comme toutes les hypothèses sont 
-   utiles (sinon on ne les inclurait pas), on pourrait remplacer [h_step] 
-   par une simple liste *)
+
+(* List of normalizations to perform : with a constructor of type 
+   [p_step] allowing to visit both left and right branches, we would be  
+   able to restrict to only one normalization by hypothesis. 
+   And since all hypothesis are useful (otherwise they wouldn't be included), 
+   we would be able to replace [h_step] by a simple list. *)
 
 Inductive h_step : Set :=
     pair_step : nat -> p_step -> h_step.
 
-(* \subsubsection{Règles pour décomposer les hypothèses} *)
-(* Ce type permet de se diriger dans les constructeurs logiques formant les
-   prédicats des hypothèses pour aller les décomposer. Ils permettent
-   en particulier d'extraire une hypothèse d'une conjonction avec
-   éventuellement le bon niveau de négations. *)
+(* \subsubsection{Rules for decomposing the hypothesis} *)
+(* This type allows to navigate in the logical constructors that 
+   form the predicats of the hypothesis in order to decompose them. 
+   This allows in particular to extract one hypothesis from a 
+   conjonction with possibly the right level of negations. *)
 
 Inductive direction : Set :=
   | D_left : direction
   | D_right : direction
   | D_mono : direction.
 
-(* Ce type permet d'extraire les composants utiles des hypothèses : que ce
-   soit des hypothèses générées par éclatement d'une disjonction, ou 
-   des équations. Le constructeur terminal indique comment résoudre le système
-   obtenu en recourrant au type de trace d'Omega [t_omega] *)
+(* This type allows to extract useful components from hypothesis, either
+   hypothesis generated by splitting a disjonction, or equations. 
+   The last constructor indicates how to solve the obtained system 
+   via the use of the trace type of Omega [t_omega] *)
 
 Inductive e_step : Set :=
   | E_SPLIT : nat -> list direction -> e_step -> e_step -> e_step
   | E_EXTRACT : nat -> list direction -> e_step -> e_step
   | E_SOLVE : t_omega -> e_step.
 
-(* \subsection{Egalité décidable efficace} *)
-(* Pour chaque type de donnée réifié, on calcule un test d'égalité efficace.
-   Ce n'est pas le cas de celui rendu par [Decide Equality].
+(* \subsection{Efficient decidable equality} *)
+(* For each reified data-type, we define an efficient equality test. 
+   It is not the one produced by [Decide Equality].
    
-   Puis on prouve deux théorèmes permettant d'éliminer de telles égalités :
+   Then we prove two theorem allowing to eliminate such equalities : 
    \begin{verbatim}
    (t1,t2: typ) (eq_typ t1 t2) = true -> t1 = t2.
    (t1,t2: typ) (eq_typ t1 t2) = false -> ~ t1 = t2.
    \end{verbatim} *)
 
-(* Ces deux tactiques permettent de résoudre pas mal de cas. L'une pour
-   les théorèmes positifs, l'autre pour les théorèmes négatifs *)
+(* \subsubsection{Reified terms} *)
 
-Ltac absurd_case := simpl in |- *; intros; discriminate.
-Ltac trivial_case := unfold not in |- *; intros; discriminate.
-
-(* \subsubsection{Entiers naturels} *)
-
-Fixpoint eq_nat (t1 t2 : nat) {struct t2} : bool :=
-  match t1 with
-  | O => match t2 with
-         | O => true
-         | _ => false
-         end
-  | S n1 => match t2 with
-            | O => false
-            | S n2 => eq_nat n1 n2
-            end
-  end.
-
-Theorem eq_nat_true : forall t1 t2 : nat, eq_nat t1 t2 = true -> t1 = t2.
-
-simple induction t1;
- [ intro t2; case t2; [ trivial | absurd_case ]
- | intros n H t2; case t2;
-    [ absurd_case
-    | simpl in |- *; intros; rewrite (H n0); [ trivial | assumption ] ] ].
-
-Qed.
-  
-Theorem eq_nat_false : forall t1 t2 : nat, eq_nat t1 t2 = false -> t1 <> t2.
-
-simple induction t1;
- [ intro t2; case t2; [ simpl in |- *; intros; discriminate | trivial_case ]
- | intros n H t2; case t2; simpl in |- *; unfold not in |- *; intros;
-    [ discriminate | elim (H n0 H0); simplify_eq H1; trivial ] ].
-
-Qed.
-                                   
-
-(* \subsubsection{Entiers positifs} *)
-
-Fixpoint eq_pos (p1 p2 : positive) {struct p2} : bool :=
-  match p1 with
-  | xI n1 => match p2 with
-             | xI n2 => eq_pos n1 n2
-             | _ => false
-             end
-  | xO n1 => match p2 with
-             | xO n2 => eq_pos n1 n2
-             | _ => false
-             end
-  | xH => match p2 with
-          | xH => true
-          | _ => false
-          end
-  end.
-
-Theorem eq_pos_true : forall t1 t2 : positive, eq_pos t1 t2 = true -> t1 = t2.
-
-simple induction t1;
- [ intros p H t2; case t2;
-    [ simpl in |- *; intros; rewrite (H p0 H0); trivial
-    | absurd_case
-    | absurd_case ]
- | intros p H t2; case t2;
-    [ absurd_case
-    | simpl in |- *; intros; rewrite (H p0 H0); trivial
-    | absurd_case ]
- | intro t2; case t2; [ absurd_case | absurd_case | auto ] ].
-
-Qed.
-  
-Theorem eq_pos_false :
- forall t1 t2 : positive, eq_pos t1 t2 = false -> t1 <> t2.
-
-simple induction t1;
- [ intros p H t2; case t2;
-    [ simpl in |- *; unfold not in |- *; intros; elim (H p0 H0);
-       simplify_eq H1; auto
-    | trivial_case
-    | trivial_case ]
- | intros p H t2; case t2;
-    [ trivial_case
-    | simpl in |- *; unfold not in |- *; intros; elim (H p0 H0);
-       simplify_eq H1; auto
-    | trivial_case ]
- | intros t2; case t2; [ trivial_case | trivial_case | absurd_case ] ].
-Qed.
-
-(* \subsubsection{Entiers relatifs} *)
-
-Definition eq_Z (z1 z2 : Z) : bool :=
-  match z1 with
-  | Z0 => match z2 with
-          | Z0 => true
-          | _ => false
-          end
-  | Zpos p1 => match z2 with
-               | Zpos p2 => eq_pos p1 p2
-               | _ => false
-               end
-  | Zneg p1 => match z2 with
-               | Zneg p2 => eq_pos p1 p2
-               | _ => false
-               end
-  end.
-
-Theorem eq_Z_true : forall t1 t2 : Z, eq_Z t1 t2 = true -> t1 = t2.
-
-simple induction t1;
- [ intros t2; case t2; [ auto | absurd_case | absurd_case ]
- | intros p t2; case t2;
-    [ absurd_case
-    | simpl in |- *; intros; rewrite (eq_pos_true p p0 H); trivial
-    | absurd_case ]
- | intros p t2; case t2;
-    [ absurd_case
-    | absurd_case
-    | simpl in |- *; intros; rewrite (eq_pos_true p p0 H); trivial ] ].
-
-Qed.
-
-Theorem eq_Z_false : forall t1 t2 : Z, eq_Z t1 t2 = false -> t1 <> t2.
-
-simple induction t1;
- [ intros t2; case t2; [ absurd_case | trivial_case | trivial_case ]
- | intros p t2; case t2;
-    [ absurd_case
-    | simpl in |- *; unfold not in |- *; intros; elim (eq_pos_false p p0 H);
-       simplify_eq H0; auto
-    | trivial_case ]
- | intros p t2; case t2;
-    [ absurd_case
-    | trivial_case
-    | simpl in |- *; unfold not in |- *; intros; elim (eq_pos_false p p0 H);
-       simplify_eq H0; auto ] ].
-Qed.
-
-(* \subsubsection{Termes réifiés} *)
+Open Scope romega_scope.
 
 Fixpoint eq_term (t1 t2 : term) {struct t2} : bool :=
-  match t1 with
-  | Tint st1 => match t2 with
-                | Tint st2 => eq_Z st1 st2
-                | _ => false
-                end
-  | (st11 + st12)%term =>
-      match t2 with
-      | (st21 + st22)%term => eq_term st11 st21 && eq_term st12 st22
-      | _ => false
-      end
-  | (st11 * st12)%term =>
-      match t2 with
-      | (st21 * st22)%term => eq_term st11 st21 && eq_term st12 st22
-      | _ => false
-      end
-  | (st11 - st12)%term =>
-      match t2 with
-      | (st21 - st22)%term => eq_term st11 st21 && eq_term st12 st22
-      | _ => false
-      end
-  | (- st1)%term =>
-      match t2 with
-      | (- st2)%term => eq_term st1 st2
-      | _ => false
-      end
-  | [st1]%term =>
-      match t2 with
-      | [st2]%term => eq_nat st1 st2
-      | _ => false
-      end
-  end.  
+  match t1, t2 with
+  | Tint st1, Tint st2 => beq st1 st2
+  | (st11 + st12), (st21 + st22) => eq_term st11 st21 && eq_term st12 st22
+  | (st11 * st12), (st21 * st22) => eq_term st11 st21 && eq_term st12 st22
+  | (st11 - st12), (st21 - st22) => eq_term st11 st21 && eq_term st12 st22
+  | (- st1), (- st2) => eq_term st1 st2
+  | [st1], [st2] => beq_nat st1 st2
+  | _, _ => false
+  end.
+
+Close Scope romega_scope.  
 
 Theorem eq_term_true : forall t1 t2 : term, eq_term t1 t2 = true -> t1 = t2.
-
-
-simple induction t1; intros until t2; case t2; try absurd_case; simpl in |- *;
- [ intros; elim eq_Z_true with (1 := H); trivial
+Proof.
+ simple induction t1; intros until t2; case t2; simpl in *;
+ try (intros; discriminate; fail); 
+ [ intros; elim beq_true with (1 := H); trivial
  | intros t21 t22 H3; elim andb_prop with (1 := H3); intros H4 H5;
     elim H with (1 := H4); elim H0 with (1 := H5); 
     trivial
@@ -417,16 +1074,17 @@ simple induction t1; intros until t2; case t2; try absurd_case; simpl in |- *;
     elim H with (1 := H4); elim H0 with (1 := H5); 
     trivial
  | intros t21 H3; elim H with (1 := H3); trivial
- | intros; elim eq_nat_true with (1 := H); trivial ].
-
+ | intros; elim beq_nat_true with (1 := H); trivial ].
 Qed.
+
+Ltac trivial_case := unfold not in |- *; intros; discriminate.
 
 Theorem eq_term_false :
  forall t1 t2 : term, eq_term t1 t2 = false -> t1 <> t2.
-
-simple induction t1;
+Proof.
+ simple induction t1;
  [ intros z t2; case t2; try trivial_case; simpl in |- *; unfold not in |- *;
-    intros; elim eq_Z_false with (1 := H); simplify_eq H0; 
+    intros; elim beq_false with (1 := H); simplify_eq H0; 
     auto
  | intros t11 H1 t12 H2 t2; case t2; try trivial_case; simpl in |- *;
     intros t21 t22 H3; unfold not in |- *; intro H4;
@@ -447,9 +1105,8 @@ simple induction t1;
     unfold not in |- *; intro H4; elim H1 with (1 := H3); 
     simplify_eq H4; auto
  | intros n t2; case t2; try trivial_case; simpl in |- *; unfold not in |- *;
-    intros; elim eq_nat_false with (1 := H); simplify_eq H0; 
+    intros; elim beq_nat_false with (1 := H); simplify_eq H0; 
     auto ].
-
 Qed.
 
 (* \subsubsection{Tactiques pour éliminer ces tests} 
@@ -463,54 +1120,29 @@ Qed.
    tel test préserve bien l'information voulue mais calculatoirement de
    telles fonctions sont trop lentes. *)
 
-(* Le théorème suivant permet de garder dans les hypothèses la valeur
-   du booléen lors de l'élimination. *)
-
-Theorem bool_ind2 :
- forall (P : bool -> Prop) (b : bool),
- (b = true -> P true) -> (b = false -> P false) -> P b.
-
-simple induction b; auto.
-Qed.
-
 (* Les tactiques définies si après se comportent exactement comme si on
    avait utilisé le test précédent et fait une elimination dessus. *)
 
 Ltac elim_eq_term t1 t2 :=
-  pattern (eq_term t1 t2) in |- *; apply bool_ind2; intro Aux;
+  pattern (eq_term t1 t2) in |- *; apply bool_eq_ind; intro Aux;
    [ generalize (eq_term_true t1 t2 Aux); clear Aux
    | generalize (eq_term_false t1 t2 Aux); clear Aux ].
 
-Ltac elim_eq_Z t1 t2 :=
-  pattern (eq_Z t1 t2) in |- *; apply bool_ind2; intro Aux;
-   [ generalize (eq_Z_true t1 t2 Aux); clear Aux
-   | generalize (eq_Z_false t1 t2 Aux); clear Aux ].
+Ltac elim_beq t1 t2 :=
+  pattern (beq t1 t2) in |- *; apply bool_eq_ind; intro Aux;
+   [ generalize (beq_true t1 t2 Aux); clear Aux
+   | generalize (beq_false t1 t2 Aux); clear Aux ].
 
-Ltac elim_eq_pos t1 t2 :=
-  pattern (eq_pos t1 t2) in |- *; apply bool_ind2; intro Aux;
-   [ generalize (eq_pos_true t1 t2 Aux); clear Aux
-   | generalize (eq_pos_false t1 t2 Aux); clear Aux ].
+Ltac elim_bgt t1 t2 := 
+  pattern (bgt t1 t2) in |- *; apply bool_eq_ind; intro Aux; 
+  [ generalize (bgt_true t1 t2 Aux); clear Aux
+  | generalize (bgt_false t1 t2 Aux); clear Aux ].
 
-(* \subsubsection{Comparaison sur Z} *)
-
-(* Sujet très lié au précédent : on introduit la tactique d'élimination
-   avec son théorème *)
-
-Theorem relation_ind2 :
- forall (P : comparison -> Prop) (b : comparison),
- (b = Eq -> P Eq) ->
- (b = Lt -> P Lt) ->
- (b = Gt -> P Gt) -> P b.
-
-simple induction b; auto.
-Qed.
-
-Ltac elim_Zcompare t1 t2 := pattern (t1 ?= t2) in |- *; apply relation_ind2.
 
 (* \subsection{Interprétations}
    \subsubsection{Interprétation des termes dans Z} *)
 
-Fixpoint interp_term (env : list Z) (t : term) {struct t} : Z :=
+Fixpoint interp_term (env : list int) (t : term) {struct t} : int :=
   match t with
   | Tint x => x
   | (t1 + t2)%term => interp_term env t1 + interp_term env t2
@@ -521,7 +1153,8 @@ Fixpoint interp_term (env : list Z) (t : term) {struct t} : Z :=
   end.
 
 (* \subsubsection{Interprétation des prédicats} *) 
-Fixpoint interp_proposition (envp : PropList) (env : list Z)
+
+Fixpoint interp_proposition (envp : list Prop) (env : list int)
  (p : proposition) {struct p} : Prop :=
   match p with
   | EqTerm t1 t2 => interp_term env t1 = interp_term env t2
@@ -532,14 +1165,14 @@ Fixpoint interp_proposition (envp : PropList) (env : list Z)
   | GeqTerm t1 t2 => interp_term env t1 >= interp_term env t2
   | GtTerm t1 t2 => interp_term env t1 > interp_term env t2
   | LtTerm t1 t2 => interp_term env t1 < interp_term env t2
-  | NeqTerm t1 t2 => Zne (interp_term env t1) (interp_term env t2)
+  | NeqTerm t1 t2 => (interp_term env t1)<>(interp_term env t2)
   | Tor p1 p2 =>
       interp_proposition envp env p1 \/ interp_proposition envp env p2
   | Tand p1 p2 =>
       interp_proposition envp env p1 /\ interp_proposition envp env p2
   | Timp p1 p2 =>
       interp_proposition envp env p1 -> interp_proposition envp env p2
-  | Tprop n => nthProp n envp True
+  | Tprop n => nth n envp True
   end.
 
 (* \subsubsection{Inteprétation des listes d'hypothèses}
@@ -547,7 +1180,7 @@ Fixpoint interp_proposition (envp : PropList) (env : list Z)
    Interprétation sous forme d'une conjonction d'hypothèses plus faciles
    à manipuler individuellement *)
 
-Fixpoint interp_hyps (envp : PropList) (env : list Z) 
+Fixpoint interp_hyps (envp : list Prop) (env : list int) 
  (l : hyps) {struct l} : Prop :=
   match l with
   | nil => True
@@ -559,8 +1192,8 @@ Fixpoint interp_hyps (envp : PropList) (env : list Z)
    [Generalize] et qu'une conjonction est forcément lourde (répétition des
    types dans les conjonctions intermédiaires) *)
 
-Fixpoint interp_goal_concl (c : proposition) (envp : PropList) 
- (env : list Z) (l : hyps) {struct l} : Prop :=
+Fixpoint interp_goal_concl (c : proposition) (envp : list Prop) 
+ (env : list int) (l : hyps) {struct l} : Prop :=
   match l with
   | nil => interp_proposition envp env c
   | p' :: l' =>
@@ -573,19 +1206,19 @@ Notation interp_goal := (interp_goal_concl FalseTerm).
    interprétations. *)
 
 Theorem goal_to_hyps :
- forall (envp : PropList) (env : list Z) (l : hyps),
+ forall (envp : list Prop) (env : list int) (l : hyps),
  (interp_hyps envp env l -> False) -> interp_goal envp env l.
-
-simple induction l;
+Proof.
+ simple induction l;
  [ simpl in |- *; auto
  | simpl in |- *; intros a l1 H1 H2 H3; apply H1; intro H4; apply H2; auto ].
 Qed.
 
 Theorem hyps_to_goal :
- forall (envp : PropList) (env : list Z) (l : hyps),
+ forall (envp : list Prop) (env : list int) (l : hyps),
  interp_goal envp env l -> interp_hyps envp env l -> False.
-
-simple induction l; simpl in |- *; [ auto | intros; apply H; elim H1; auto ].
+Proof.
+ simple induction l; simpl in |- *; [ auto | intros; apply H; elim H1; auto ].
 Qed.
       
 (* \subsection{Manipulations sur les hypothèses} *)
@@ -593,7 +1226,7 @@ Qed.
 (* \subsubsection{Définitions de base de stabilité pour la réflexion} *)
 (* Une opération laisse un terme stable si l'égalité est préservée *)
 Definition term_stable (f : term -> term) :=
-  forall (e : list Z) (t : term), interp_term e t = interp_term e (f t).
+  forall (e : list int) (t : term), interp_term e t = interp_term e (f t).
 
 (* Une opération est valide sur une hypothèse, si l'hypothèse implique le
    résultat de l'opération. \emph{Attention : cela ne concerne que des 
@@ -602,11 +1235,11 @@ Definition term_stable (f : term -> term) :=
    en argument (cela suffit pour omega). *)
 
 Definition valid1 (f : proposition -> proposition) :=
-  forall (ep : PropList) (e : list Z) (p1 : proposition),
+  forall (ep : list Prop) (e : list int) (p1 : proposition),
   interp_proposition ep e p1 -> interp_proposition ep e (f p1).
 
 Definition valid2 (f : proposition -> proposition -> proposition) :=
-  forall (ep : PropList) (e : list Z) (p1 p2 : proposition),
+  forall (ep : list Prop) (e : list int) (p1 p2 : proposition),
   interp_proposition ep e p1 ->
   interp_proposition ep e p2 -> interp_proposition ep e (f p1 p2).
 
@@ -615,31 +1248,31 @@ Definition valid2 (f : proposition -> proposition -> proposition) :=
    On reste contravariant *)
 
 Definition valid_hyps (f : hyps -> hyps) :=
-  forall (ep : PropList) (e : list Z) (lp : hyps),
+  forall (ep : list Prop) (e : list int) (lp : hyps),
   interp_hyps ep e lp -> interp_hyps ep e (f lp).
 
 (* Enfin ce théorème élimine la contravariance et nous ramène à une 
    opération sur les buts *)
 
- Theorem valid_goal :
-  forall (ep : PropList) (env : list Z) (l : hyps) (a : hyps -> hyps),
+Theorem valid_goal :
+  forall (ep : list Prop) (env : list int) (l : hyps) (a : hyps -> hyps),
   valid_hyps a -> interp_goal ep env (a l) -> interp_goal ep env l.
-
-intros; simpl in |- *; apply goal_to_hyps; intro H1;
+Proof.
+ intros; simpl in |- *; apply goal_to_hyps; intro H1;
  apply (hyps_to_goal ep env (a l) H0); apply H; assumption.
 Qed.
 
 (* \subsubsection{Généralisation a des listes de buts (disjonctions)} *)
 
 
-Fixpoint interp_list_hyps (envp : PropList) (env : list Z) 
+Fixpoint interp_list_hyps (envp : list Prop) (env : list int) 
  (l : lhyps) {struct l} : Prop :=
   match l with
   | nil => False
   | h :: l' => interp_hyps envp env h \/ interp_list_hyps envp env l'
   end.
 
-Fixpoint interp_list_goal (envp : PropList) (env : list Z) 
+Fixpoint interp_list_goal (envp : list Prop) (env : list int) 
  (l : lhyps) {struct l} : Prop :=
   match l with
   | nil => True
@@ -647,10 +1280,10 @@ Fixpoint interp_list_goal (envp : PropList) (env : list Z)
   end.
 
 Theorem list_goal_to_hyps :
- forall (envp : PropList) (env : list Z) (l : lhyps),
+ forall (envp : list Prop) (env : list int) (l : lhyps),
  (interp_list_hyps envp env l -> False) -> interp_list_goal envp env l.
-
-simple induction l; simpl in |- *;
+Proof.
+ simple induction l; simpl in |- *;
  [ auto
  | intros h1 l1 H H1; split;
     [ apply goal_to_hyps; intro H2; apply H1; auto
@@ -658,37 +1291,37 @@ simple induction l; simpl in |- *;
 Qed.
 
 Theorem list_hyps_to_goal :
- forall (envp : PropList) (env : list Z) (l : lhyps),
+ forall (envp : list Prop) (env : list int) (l : lhyps),
  interp_list_goal envp env l -> interp_list_hyps envp env l -> False.
-
-simple induction l; simpl in |- *;
+Proof.
+ simple induction l; simpl in |- *;
  [ auto
  | intros h1 l1 H (H1, H2) H3; elim H3; intro H4;
     [ apply hyps_to_goal with (1 := H1); assumption | auto ] ].
 Qed.
 
 Definition valid_list_hyps (f : hyps -> lhyps) :=
-  forall (ep : PropList) (e : list Z) (lp : hyps),
+  forall (ep : list Prop) (e : list int) (lp : hyps),
   interp_hyps ep e lp -> interp_list_hyps ep e (f lp).
 
 Definition valid_list_goal (f : hyps -> lhyps) :=
-  forall (ep : PropList) (e : list Z) (lp : hyps),
+  forall (ep : list Prop) (e : list int) (lp : hyps),
   interp_list_goal ep e (f lp) -> interp_goal ep e lp.
 
 Theorem goal_valid :
  forall f : hyps -> lhyps, valid_list_hyps f -> valid_list_goal f.
-
-unfold valid_list_goal in |- *; intros f H ep e lp H1; apply goal_to_hyps;
+Proof.
+ unfold valid_list_goal in |- *; intros f H ep e lp H1; apply goal_to_hyps;
  intro H2; apply list_hyps_to_goal with (1 := H1); 
  apply (H ep e lp); assumption.
 Qed.
  
 Theorem append_valid :
- forall (ep : PropList) (e : list Z) (l1 l2 : lhyps),
+ forall (ep : list Prop) (e : list int) (l1 l2 : lhyps),
  interp_list_hyps ep e l1 \/ interp_list_hyps ep e l2 ->
  interp_list_hyps ep e (l1 ++ l2).
-
-intros ep e; simple induction l1;
+Proof.
+ intros ep e; simple induction l1;
  [ simpl in |- *; intros l2 [H| H]; [ contradiction | trivial ]
  | simpl in |- *; intros h1 t1 HR l2 [[H| H]| H];
     [ auto
@@ -703,10 +1336,10 @@ Qed.
 Definition nth_hyps (n : nat) (l : hyps) := nth n l TrueTerm.
 
 Theorem nth_valid :
- forall (ep : PropList) (e : list Z) (i : nat) (l : hyps),
+ forall (ep : list Prop) (e : list int) (i : nat) (l : hyps),
  interp_hyps ep e l -> interp_proposition ep e (nth_hyps i l).
-
-unfold nth_hyps in |- *; simple induction i;
+Proof.
+ unfold nth_hyps in |- *; simple induction i;
  [ simple induction l; simpl in |- *; [ auto | intros; elim H0; auto ]
  | intros n H; simple induction l;
     [ simpl in |- *; trivial
@@ -722,8 +1355,8 @@ Definition apply_oper_2 (i j : nat)
 Theorem apply_oper_2_valid :
  forall (i j : nat) (f : proposition -> proposition -> proposition),
  valid2 f -> valid_hyps (apply_oper_2 i j f).
-
-intros i j f Hf; unfold apply_oper_2, valid_hyps in |- *; simpl in |- *;
+Proof.
+ intros i j f Hf; unfold apply_oper_2, valid_hyps in |- *; simpl in |- *;
  intros lp Hlp; split; [ apply Hf; apply nth_valid; assumption | assumption ].
 Qed.
 
@@ -743,8 +1376,8 @@ Fixpoint apply_oper_1 (i : nat) (f : proposition -> proposition)
 Theorem apply_oper_1_valid :
  forall (i : nat) (f : proposition -> proposition),
  valid1 f -> valid_hyps (apply_oper_1 i f).
-
-unfold valid_hyps in |- *; intros i f Hf ep e; elim i;
+Proof.
+ unfold valid_hyps in |- *; intros i f Hf ep e; elim i;
  [ intro lp; case lp;
     [ simpl in |- *; trivial
     | simpl in |- *; intros p l' (H1, H2); split;
@@ -753,7 +1386,6 @@ unfold valid_hyps in |- *; intros i f Hf ep e; elim i;
     [ simpl in |- *; auto
     | simpl in |- *; intros p l' (H1, H2); split;
        [ assumption | apply Hrec; assumption ] ] ].
-
 Qed.
 
 (* \subsubsection{Manipulations de termes} *)
@@ -789,31 +1421,31 @@ Definition apply_both (f g : term -> term) (t : term) :=
 
 Theorem apply_left_stable :
  forall f : term -> term, term_stable f -> term_stable (apply_left f).
-
-unfold term_stable in |- *; intros f H e t; case t; auto; simpl in |- *;
+Proof.
+ unfold term_stable in |- *; intros f H e t; case t; auto; simpl in |- *;
  intros; elim H; trivial.
 Qed.
 
 Theorem apply_right_stable :
  forall f : term -> term, term_stable f -> term_stable (apply_right f).
-
-unfold term_stable in |- *; intros f H e t; case t; auto; simpl in |- *;
+Proof.
+ unfold term_stable in |- *; intros f H e t; case t; auto; simpl in |- *;
  intros t0 t1; elim H; trivial.
 Qed.
 
 Theorem apply_both_stable :
  forall f g : term -> term,
  term_stable f -> term_stable g -> term_stable (apply_both f g).
-
-unfold term_stable in |- *; intros f g H1 H2 e t; case t; auto; simpl in |- *;
+Proof.
+ unfold term_stable in |- *; intros f g H1 H2 e t; case t; auto; simpl in |- *;
  intros t0 t1; elim H1; elim H2; trivial.
 Qed.
 
 Theorem compose_term_stable :
  forall f g : term -> term,
  term_stable f -> term_stable g -> term_stable (fun t : term => f (g t)).
-
-unfold term_stable in |- *; intros f g Hf Hg e t; elim Hf; apply Hg.
+Proof.
+ unfold term_stable in |- *; intros f g Hf Hg e t; elim Hf; apply Hg.
 Qed.
 
 (* \subsection{Les règles de réécriture} *)
@@ -879,21 +1511,7 @@ Ltac loop t :=
     | Tand x x0 => _
     | Timp x x0 => _
     | Tprop x => _
-    end =>
-       case X1;
-       [ intro; intro
-       | intro; intro
-       | idtac
-       | idtac
-       | intro
-       | intro; intro
-       | intro; intro
-       | intro; intro
-       | intro; intro
-       | intro; intro
-       | intro; intro
-       | intro; intro
-       | intro ]; auto; Simplify
+    end => destruct X1; auto; Simplify
   | match ?X1 with
     | Tint x => _
     | (x + x0)%term => _
@@ -901,38 +1519,27 @@ Ltac loop t :=
     | (x - x0)%term => _
     | (- x)%term => _
     | [x]%term => _
-    end =>
-      case X1;
-       [ intro | intro; intro | intro; intro | intro; intro | intro | intro ];
-       auto; Simplify
-  | match ?X1 ?= ?X2 with
-    | Eq => _
-    | Lt => _
-    | Gt => _
-    end =>
-      elim_Zcompare X1 X2; intro; auto; Simplify
-  | match ?X1 with
-    | Z0 => _
-    | Zpos x => _
-    | Zneg x => _
-    end =>
-      case X1; [ idtac | intro | intro ]; auto; Simplify
-  | (if eq_Z ?X1 ?X2 then _ else _) =>
-      elim_eq_Z X1 X2; intro H; [ rewrite H; clear H | clear H ];
+    end => destruct X1; auto; Simplify
+  | (if beq ?X1 ?X2 then _ else _) =>
+      let H := fresh "H" in 
+      elim_beq X1 X2; intro H; try (rewrite H in *; clear H);
        simpl in |- *; auto; Simplify
+  | (if bgt ?X1 ?X2 then _ else _) =>
+      let H := fresh "H" in 
+      elim_bgt X1 X2; intro H; simpl in |- *; auto; Simplify
   | (if eq_term ?X1 ?X2 then _ else _) =>
-      elim_eq_term X1 X2; intro H; [ rewrite H; clear H | clear H ];
+      let H := fresh "H" in 
+      elim_eq_term X1 X2; intro H; try (rewrite H in *; clear H); 
        simpl in |- *; auto; Simplify
-  | (if eq_pos ?X1 ?X2 then _ else _) =>
-      elim_eq_pos X1 X2; intro H; [ rewrite H; clear H | clear H ];
-       simpl in |- *; auto; Simplify
+  | (if _ && _ then _ else _) => rewrite andb_if; Simplify
+  | (if negb _ then _ else _) => rewrite negb_if; Simplify
   | _ => fail
   end
- with Simplify := match goal with
-                  |  |- ?X1 => try loop X1
-                  | _ => idtac
-                  end.
 
+with Simplify := match goal with
+  |  |- ?X1 => try loop X1
+  | _ => idtac
+  end.
 
 Ltac prove_stable x th :=
   match constr:x with
@@ -949,8 +1556,8 @@ Definition Tplus_assoc_l (t : term) :=
   end.
 
 Theorem Tplus_assoc_l_stable : term_stable Tplus_assoc_l.
-
-prove_stable Tplus_assoc_l Zplus_assoc.
+Proof.
+ prove_stable Tplus_assoc_l (ring.(Radd_assoc)).
 Qed.
 
 Definition Tplus_assoc_r (t : term) :=
@@ -960,8 +1567,8 @@ Definition Tplus_assoc_r (t : term) :=
   end.
 
 Theorem Tplus_assoc_r_stable : term_stable Tplus_assoc_r.
-
-prove_stable Tplus_assoc_r Zplus_assoc_reverse.
+Proof.
+ prove_stable Tplus_assoc_r plus_assoc_reverse.
 Qed.
 
 Definition Tmult_assoc_r (t : term) :=
@@ -971,8 +1578,8 @@ Definition Tmult_assoc_r (t : term) :=
   end.
 
 Theorem Tmult_assoc_r_stable : term_stable Tmult_assoc_r.
-
-prove_stable Tmult_assoc_r Zmult_assoc_reverse.
+Proof.
+ prove_stable Tmult_assoc_r mult_assoc_reverse.
 Qed.
 
 Definition Tplus_permute (t : term) :=
@@ -982,8 +1589,8 @@ Definition Tplus_permute (t : term) :=
   end.
 
 Theorem Tplus_permute_stable : term_stable Tplus_permute.
-
-prove_stable Tplus_permute Zplus_permute.
+Proof.
+ prove_stable Tplus_permute plus_permute.
 Qed.
 
 Definition Tplus_comm (t : term) :=
@@ -993,8 +1600,8 @@ Definition Tplus_comm (t : term) :=
   end.
 
 Theorem Tplus_comm_stable : term_stable Tplus_comm.
-
-prove_stable Tplus_comm Zplus_comm.
+Proof.
+ prove_stable Tplus_comm plus_comm.
 Qed.
 
 Definition Tmult_comm (t : term) :=
@@ -1004,24 +1611,22 @@ Definition Tmult_comm (t : term) :=
   end.
 
 Theorem Tmult_comm_stable : term_stable Tmult_comm.
-
-prove_stable Tmult_comm Zmult_comm.
+Proof.
+ prove_stable Tmult_comm mult_comm.
 Qed.
 
 Definition T_OMEGA10 (t : term) :=
   match t with
   | ((v * Tint c1 + l1) * Tint k1 + (v' * Tint c2 + l2) * Tint k2)%term =>
-      match eq_term v v' with
-      | true =>
-          (v * Tint (c1 * k1 + c2 * k2) + (l1 * Tint k1 + l2 * Tint k2))%term
-      | false => t
-      end
+      if eq_term v v' 
+      then (v * Tint (c1 * k1 + c2 * k2)%I + (l1 * Tint k1 + l2 * Tint k2))%term
+      else t
   | _ => t
   end.
 
 Theorem T_OMEGA10_stable : term_stable T_OMEGA10.
-
-prove_stable T_OMEGA10 OMEGA10.
+Proof.
+ prove_stable T_OMEGA10 OMEGA10.
 Qed.
 
 Definition T_OMEGA11 (t : term) :=
@@ -1032,8 +1637,8 @@ Definition T_OMEGA11 (t : term) :=
   end.
 
 Theorem T_OMEGA11_stable : term_stable T_OMEGA11.
-
-prove_stable T_OMEGA11 OMEGA11.
+Proof.
+ prove_stable T_OMEGA11 OMEGA11.
 Qed.
 
 Definition T_OMEGA12 (t : term) :=
@@ -1044,52 +1649,37 @@ Definition T_OMEGA12 (t : term) :=
   end.
 
 Theorem T_OMEGA12_stable : term_stable T_OMEGA12.
-
-prove_stable T_OMEGA12 OMEGA12.
+Proof.
+ prove_stable T_OMEGA12 OMEGA12.
 Qed. 
 
 Definition T_OMEGA13 (t : term) :=
   match t with
-  | (v * Tint (Zpos x) + l1 + (v' * Tint (Zneg x') + l2))%term =>
-      match eq_term v v' with
-      | true =>
-          match eq_pos x x' with
-          | true => (l1 + l2)%term
-          | false => t
-          end
-      | false => t
-      end
-  | (v * Tint (Zneg x) + l1 + (v' * Tint (Zpos x') + l2))%term =>
-      match eq_term v v' with
-      | true =>
-          match eq_pos x x' with
-          | true => (l1 + l2)%term
-          | false => t
-          end
-      | false => t
-      end
+  | (v * Tint x + l1 + (v' * Tint x' + l2))%term =>
+      if eq_term v v' && beq x (-x') 
+      then (l1+l2)%term
+      else t
   | _ => t
   end.
 
 Theorem T_OMEGA13_stable : term_stable T_OMEGA13.
-
-unfold term_stable, T_OMEGA13 in |- *; intros; Simplify; simpl in |- *;
- [ apply OMEGA13 | apply OMEGA14 ].
+Proof.
+ unfold term_stable, T_OMEGA13 in |- *; intros; Simplify; simpl in |- *;
+ apply OMEGA13.
 Qed.
 
 Definition T_OMEGA15 (t : term) :=
   match t with
   | (v * Tint c1 + l1 + (v' * Tint c2 + l2) * Tint k2)%term =>
-      match eq_term v v' with
-      | true => (v * Tint (c1 + c2 * k2) + (l1 + l2 * Tint k2))%term
-      | false => t
-      end
+      if eq_term v v' 
+      then (v * Tint (c1 + c2 * k2)%I + (l1 + l2 * Tint k2))%term
+      else t
   | _ => t
   end.
 
 Theorem T_OMEGA15_stable : term_stable T_OMEGA15.
-
-prove_stable T_OMEGA15 OMEGA15.
+Proof.
+ prove_stable T_OMEGA15 OMEGA15.
 Qed.
 
 Definition T_OMEGA16 (t : term) :=
@@ -1100,20 +1690,19 @@ Definition T_OMEGA16 (t : term) :=
 
 
 Theorem T_OMEGA16_stable : term_stable T_OMEGA16.
-
-prove_stable T_OMEGA16 OMEGA16.
+Proof.
+ prove_stable T_OMEGA16 OMEGA16.
 Qed.
 
 Definition Tred_factor5 (t : term) :=
   match t with
-  | (x * Tint Z0 + y)%term => y
+  | (x * Tint c + y)%term => if beq c 0 then y else t
   | _ => t
   end.
 
 Theorem Tred_factor5_stable : term_stable Tred_factor5.
-
-
-prove_stable Tred_factor5 Zred_factor5.
+Proof.
+ prove_stable Tred_factor5 red_factor5.
 Qed.
 
 Definition Topp_plus (t : term) :=
@@ -1123,8 +1712,8 @@ Definition Topp_plus (t : term) :=
   end.
 
 Theorem Topp_plus_stable : term_stable Topp_plus.
-
-prove_stable Topp_plus Zopp_plus_distr.
+Proof.
+ prove_stable Topp_plus opp_plus_distr.
 Qed.
 
 
@@ -1135,8 +1724,8 @@ Definition Topp_opp (t : term) :=
   end.
 
 Theorem Topp_opp_stable : term_stable Topp_opp.
-
-prove_stable Topp_opp Zopp_involutive.
+Proof.
+ prove_stable Topp_opp opp_involutive.
 Qed.
 
 Definition Topp_mult_r (t : term) :=
@@ -1146,19 +1735,19 @@ Definition Topp_mult_r (t : term) :=
   end.
 
 Theorem Topp_mult_r_stable : term_stable Topp_mult_r.
-
-prove_stable Topp_mult_r Zopp_mult_distr_r.
+Proof.
+ prove_stable Topp_mult_r opp_mult_distr_r.
 Qed.
 
 Definition Topp_one (t : term) :=
   match t with
-  | (- x)%term => (x * Tint (-1))%term
+  | (- x)%term => (x * Tint (-(1)))%term
   | _ => t
   end.
 
 Theorem Topp_one_stable : term_stable Topp_one.
-
-prove_stable Topp_one Zopp_eq_mult_neg_1.
+Proof.
+ prove_stable Topp_one opp_eq_mult_neg_1.
 Qed.
 
 Definition Tmult_plus_distr (t : term) :=
@@ -1168,8 +1757,8 @@ Definition Tmult_plus_distr (t : term) :=
   end.
 
 Theorem Tmult_plus_distr_stable : term_stable Tmult_plus_distr.
-
-prove_stable Tmult_plus_distr Zmult_plus_distr_l.
+Proof.
+ prove_stable Tmult_plus_distr mult_plus_distr_r.
 Qed.
 
 Definition Tmult_opp_left (t : term) :=
@@ -1179,8 +1768,8 @@ Definition Tmult_opp_left (t : term) :=
   end.
 
 Theorem Tmult_opp_left_stable : term_stable Tmult_opp_left.
-
-prove_stable Tmult_opp_left Zmult_opp_comm.
+Proof.
+ prove_stable Tmult_opp_left mult_opp_comm.
 Qed.
 
 Definition Tmult_assoc_reduced (t : term) :=
@@ -1190,90 +1779,80 @@ Definition Tmult_assoc_reduced (t : term) :=
   end.
 
 Theorem Tmult_assoc_reduced_stable : term_stable Tmult_assoc_reduced.
-
-prove_stable Tmult_assoc_reduced Zmult_assoc_reverse.
+Proof.
+ prove_stable Tmult_assoc_reduced mult_assoc_reverse.
 Qed.
 
 Definition Tred_factor0 (t : term) := (t * Tint 1)%term.
 
 Theorem Tred_factor0_stable : term_stable Tred_factor0.
-
-prove_stable Tred_factor0 Zred_factor0.
+Proof.
+ prove_stable Tred_factor0 red_factor0.
 Qed.
 
 Definition Tred_factor1 (t : term) :=
   match t with
   | (x + y)%term =>
-      match eq_term x y with
-      | true => (x * Tint 2)%term
-      | false => t
-      end
+      if eq_term x y 
+      then (x * Tint 2)%term
+      else t 
   | _ => t
   end.
 
 Theorem Tred_factor1_stable : term_stable Tred_factor1.
-
-prove_stable Tred_factor1 Zred_factor1.
+Proof.
+ prove_stable Tred_factor1 red_factor1.
 Qed.
 
 Definition Tred_factor2 (t : term) :=
   match t with
   | (x + y * Tint k)%term =>
-      match eq_term x y with
-      | true => (x * Tint (1 + k))%term
-      | false => t
-      end
+      if eq_term x y 
+      then (x * Tint (1 + k))%term
+      else t
   | _ => t
   end.
 
-(* Attention : il faut rendre opaque [Zplus] pour éviter que la tactique
-   de simplification n'aille trop loin et défasse [Zplus 1 k] *)
-
-Opaque Zplus.
-
 Theorem Tred_factor2_stable : term_stable Tred_factor2.
-prove_stable Tred_factor2 Zred_factor2.
+Proof.
+ prove_stable Tred_factor2 red_factor2.
 Qed.
 
 Definition Tred_factor3 (t : term) :=
   match t with
   | (x * Tint k + y)%term =>
-      match eq_term x y with
-      | true => (x * Tint (1 + k))%term
-      | false => t
-      end
+      if eq_term x y 
+      then (x * Tint (1 + k))%term
+      else t
   | _ => t
   end.
 
 Theorem Tred_factor3_stable : term_stable Tred_factor3.
-
-prove_stable Tred_factor3 Zred_factor3.
+Proof.
+ prove_stable Tred_factor3 red_factor3.
 Qed.
 
 
 Definition Tred_factor4 (t : term) :=
   match t with
   | (x * Tint k1 + y * Tint k2)%term =>
-      match eq_term x y with
-      | true => (x * Tint (k1 + k2))%term
-      | false => t
-      end
+      if eq_term x y 
+      then (x * Tint (k1 + k2))%term
+      else t
   | _ => t
   end.
 
 Theorem Tred_factor4_stable : term_stable Tred_factor4.
-
-prove_stable Tred_factor4 Zred_factor4.
+Proof.
+ prove_stable Tred_factor4 red_factor4.
 Qed.
 
 Definition Tred_factor6 (t : term) := (t + Tint 0)%term.
 
 Theorem Tred_factor6_stable : term_stable Tred_factor6.
-
-prove_stable Tred_factor6 Zred_factor6.
+Proof.
+ prove_stable Tred_factor6 red_factor6.
 Qed.
-
-Transparent Zplus.
 
 Definition Tminus_def (t : term) :=
   match t with
@@ -1282,9 +1861,8 @@ Definition Tminus_def (t : term) :=
   end.
 
 Theorem Tminus_def_stable : term_stable Tminus_def.
-
-(* Le théorème ne sert à rien. Le but est prouvé avant. *)
-prove_stable Tminus_def False.
+Proof.
+ prove_stable Tminus_def minus_def.
 Qed.
 
 (* \subsection{Fonctions de réécriture complexes} *)
@@ -1332,8 +1910,8 @@ Fixpoint reduce (t : term) : term :=
   end.
 
 Theorem reduce_stable : term_stable reduce.
-
-unfold term_stable in |- *; intros e t; elim t; auto;
+Proof.
+ unfold term_stable in |- *; intros e t; elim t; auto;
  try
   (intros t0 H0 t1 H1; simpl in |- *; rewrite H0; rewrite H1;
     (case (reduce t0);
@@ -1366,8 +1944,8 @@ Fixpoint fusion (trace : list t_fusion) (t : term) {struct trace} : term :=
   end.
     
 Theorem fusion_stable : forall t : list t_fusion, term_stable (fusion t).
-
-simple induction t; simpl in |- *;
+Proof.
+ simple induction t; simpl in |- *;
  [ exact reduce_stable
  | intros stp l H; case stp;
     [ apply compose_term_stable;
@@ -1378,7 +1956,6 @@ simple induction t; simpl in |- *;
        [ apply apply_right_stable; assumption | exact T_OMEGA11_stable ]
     | apply compose_term_stable;
        [ apply apply_right_stable; assumption | exact T_OMEGA12_stable ] ] ].
-
 Qed.
 
 (* \paragraph{Fusion de deux équations dont une sans coefficient} *)
@@ -1405,8 +1982,8 @@ Fixpoint fusion_cancel (trace : nat) (t : term) {struct trace} : term :=
   end.
 
 Theorem fusion_cancel_stable : forall t : nat, term_stable (fusion_cancel t).
-
-unfold term_stable, fusion_cancel in |- *; intros trace e; elim trace;
+Proof.
+ unfold term_stable, fusion_cancel in |- *; intros trace e; elim trace;
  [ exact (reduce_stable e)
  | intros n H t; elim H; exact (T_OMEGA13_stable e t) ].
 Qed. 
@@ -1422,8 +1999,8 @@ Fixpoint scalar_norm_add (trace : nat) (t : term) {struct trace} : term :=
 
 Theorem scalar_norm_add_stable :
  forall t : nat, term_stable (scalar_norm_add t).
-
-unfold term_stable, scalar_norm_add in |- *; intros trace; elim trace;
+Proof.
+ unfold term_stable, scalar_norm_add in |- *; intros trace; elim trace;
  [ exact reduce_stable
  | intros n H e t; elim apply_right_stable;
     [ exact (T_OMEGA11_stable e t) | exact H ] ].
@@ -1437,8 +2014,8 @@ Fixpoint scalar_norm (trace : nat) (t : term) {struct trace} : term :=
   end.
 
 Theorem scalar_norm_stable : forall t : nat, term_stable (scalar_norm t).
-
-unfold term_stable, scalar_norm in |- *; intros trace; elim trace;
+Proof.
+ unfold term_stable, scalar_norm in |- *; intros trace; elim trace;
  [ exact reduce_stable
  | intros n H e t; elim apply_right_stable;
     [ exact (T_OMEGA16_stable e t) | exact H ] ].
@@ -1452,8 +2029,8 @@ Fixpoint add_norm (trace : nat) (t : term) {struct trace} : term :=
   end.
 
 Theorem add_norm_stable : forall t : nat, term_stable (add_norm t).
-
-unfold term_stable, add_norm in |- *; intros trace; elim trace;
+Proof.
+ unfold term_stable, add_norm in |- *; intros trace; elim trace;
  [ exact reduce_stable
  | intros n H e t; elim apply_right_stable;
     [ exact (Tplus_assoc_r_stable e t) | exact H ] ].
@@ -1494,8 +2071,8 @@ Fixpoint rewrite (s : step) : term -> term :=
   end.
 
 Theorem rewrite_stable : forall s : step, term_stable (rewrite s).
-
-simple induction s; simpl in |- *;
+Proof.
+ simple induction s; simpl in |- *;
  [ intros; apply apply_both_stable; auto
  | intros; apply apply_left_stable; auto
  | intros; apply apply_right_stable; auto
@@ -1532,20 +2109,18 @@ Qed.
 
 Definition constant_not_nul (i : nat) (h : hyps) :=
   match nth_hyps i h with
-  | EqTerm (Tint Z0) (Tint n) =>
-      match eq_Z n 0 with
-      | true => h
-      | false => absurd
-      end
+  | EqTerm (Tint Nul) (Tint n) =>
+      if beq n Nul then h else absurd
   | _ => h
   end.
 
 Theorem constant_not_nul_valid :
  forall i : nat, valid_hyps (constant_not_nul i).
-
-unfold valid_hyps, constant_not_nul in |- *; intros;
- generalize (nth_valid ep e i lp); Simplify; simpl in |- *;
- elim_eq_Z ipattern:z0 0; auto; simpl in |- *; intros H1 H2; 
+Proof.
+ unfold valid_hyps, constant_not_nul in |- *; intros;
+ generalize (nth_valid ep e i lp); Simplify; simpl in |- *. 
+ 
+ elim_beq i1 i0; auto; simpl in |- *; intros H1 H2; 
  elim H1; symmetry  in |- *; auto.
 Qed.   
 
@@ -1553,66 +2128,55 @@ Qed.
 
 Definition constant_neg (i : nat) (h : hyps) :=
   match nth_hyps i h with
-  | LeqTerm (Tint Z0) (Tint (Zneg n)) => absurd
+  | LeqTerm (Tint Nul) (Tint Neg) => 
+     if bgt Nul Neg then absurd else h
   | _ => h
   end.
 
 Theorem constant_neg_valid : forall i : nat, valid_hyps (constant_neg i).
-
-unfold valid_hyps, constant_neg in |- *; intros;
- generalize (nth_valid ep e i lp); Simplify; simpl in |- *;
- unfold Zle in |- *; simpl in |- *; intros H1; elim H1;
- [ assumption | trivial ].
-Qed.   
+Proof.
+ unfold valid_hyps, constant_neg in |- *; intros;
+ generalize (nth_valid ep e i lp); Simplify; simpl in |- *.
+ rewrite gt_lt_iff in H0; rewrite le_lt_iff; intuition.
+Qed.
 
 (* \paragraph{[NOT_EXACT_DIVIDE]} *)
-Definition not_exact_divide (k1 k2 : Z) (body : term) 
+Definition not_exact_divide (k1 k2 : int) (body : term) 
   (t i : nat) (l : hyps) :=
   match nth_hyps i l with
-  | EqTerm (Tint Z0) b =>
-      match
-        eq_term (scalar_norm_add t (body * Tint k1 + Tint k2)%term) b
-      with
-      | true =>
-          match k2 ?= 0 with
-          | Gt =>
-              match k1 ?= k2 with
-              | Gt => absurd
-              | _ => l
-              end
-          | _ => l
-          end
-      | false => l
-      end
+  | EqTerm (Tint Nul) b =>
+      if beq Nul 0 && 
+         eq_term (scalar_norm_add t (body * Tint k1 + Tint k2)%term) b && 
+         bgt k2 0 && 
+         bgt k1 k2 
+      then absurd
+      else l
   | _ => l
   end.
 
 Theorem not_exact_divide_valid :
- forall (k1 k2 : Z) (body : term) (t i : nat),
+ forall (k1 k2 : int) (body : term) (t i : nat),
  valid_hyps (not_exact_divide k1 k2 body t i).
-
-unfold valid_hyps, not_exact_divide in |- *; intros;
- generalize (nth_valid ep e i lp); Simplify;
- elim_eq_term (scalar_norm_add t (body * Tint k1 + Tint k2)%term) t1; 
- auto; Simplify; intro H2; elim H2; simpl in |- *;
- elim (scalar_norm_add_stable t e); simpl in |- *; 
- intro H4; absurd (interp_term e body * k1 + k2 = 0);
- [ apply OMEGA4; assumption | symmetry  in |- *; auto ].
-
+Proof.
+ unfold valid_hyps, not_exact_divide in |- *; intros;
+ generalize (nth_valid ep e i lp); Simplify.
+ rewrite (scalar_norm_add_stable t e), <-H0.
+ do 2 rewrite <- scalar_norm_add_stable; simpl in *; intros.
+ absurd (interp_term e body * k1 + k2 = 0); 
+ [ now apply OMEGA4 | symmetry; auto ].
 Qed.
 
 (* \paragraph{[O_CONTRADICTION]} *)
 
 Definition contradiction (t i j : nat) (l : hyps) :=
   match nth_hyps i l with
-  | LeqTerm (Tint Z0) b1 =>
+  | LeqTerm (Tint Nul) b1 =>
       match nth_hyps j l with
-      | LeqTerm (Tint Z0) b2 =>
+      | LeqTerm (Tint Nul') b2 =>
           match fusion_cancel t (b1 + b2)%term with
-          | Tint k => match 0 ?= k with
-                      | Gt => absurd
-                      | _ => l
-                      end
+          | Tint k => if beq Nul 0 && beq Nul' 0 && bgt 0 k 
+                      then absurd 
+                      else l
           | _ => l
           end
       | _ => l
@@ -1622,43 +2186,40 @@ Definition contradiction (t i j : nat) (l : hyps) :=
 
 Theorem contradiction_valid :
  forall t i j : nat, valid_hyps (contradiction t i j).
-
-unfold valid_hyps, contradiction in |- *; intros t i j ep e l H;
+Proof.
+ unfold valid_hyps, contradiction in |- *; intros t i j ep e l H;
  generalize (nth_valid _ _ i _ H); generalize (nth_valid _ _ j _ H);
  case (nth_hyps i l); auto; intros t1 t2; case t1; 
- auto; intros z; case z; auto; case (nth_hyps j l); 
- auto; intros t3 t4; case t3; auto; intros z'; case z'; 
- auto; simpl in |- *; intros H1 H2;
+ auto; case (nth_hyps j l); 
+ auto; intros t3 t4; case t3; auto; 
+ simpl in |- *; intros z z' H1 H2;
  generalize (refl_equal (interp_term e (fusion_cancel t (t2 + t4)%term)));
  pattern (fusion_cancel t (t2 + t4)%term) at 2 3 in |- *;
  case (fusion_cancel t (t2 + t4)%term); simpl in |- *; 
- auto; intro k; elim (fusion_cancel_stable t); simpl in |- *; 
- intro E; generalize (OMEGA2 _ _ H2 H1); rewrite E; 
- case k; auto; unfold Zle in |- *; simpl in |- *; intros p H3; 
- elim H3; auto.
-
+ auto; intro k; elim (fusion_cancel_stable t); simpl in |- *.
+ Simplify; intro H3.
+ generalize (OMEGA2 _ _ H2 H1); rewrite H3. 
+ rewrite gt_lt_iff in H0; rewrite le_lt_iff; intuition.
 Qed.
 
 (* \paragraph{[O_NEGATE_CONTRADICT]} *)
 
 Definition negate_contradict (i1 i2 : nat) (h : hyps) :=
   match nth_hyps i1 h with
-  | EqTerm (Tint Z0) b1 =>
+  | EqTerm (Tint Nul) b1 =>
       match nth_hyps i2 h with
-      | NeqTerm (Tint Z0) b2 =>
-          match eq_term b1 b2 with
-          | true => absurd
-          | false => h
-          end
+      | NeqTerm (Tint Nul') b2 =>
+          if beq Nul 0 && beq Nul' 0 && eq_term b1 b2 
+          then absurd 
+          else h
       | _ => h
       end
-  | NeqTerm (Tint Z0) b1 =>
+  | NeqTerm (Tint Nul) b1 =>
       match nth_hyps i2 h with
-      | EqTerm (Tint Z0) b2 =>
-          match eq_term b1 b2 with
-          | true => absurd
-          | false => h
-          end
+      | EqTerm (Tint Nul') b2 =>
+          if beq Nul 0 && beq Nul' 0 && eq_term b1 b2 
+          then absurd 
+          else h 
       | _ => h
       end
   | _ => h
@@ -1666,22 +2227,22 @@ Definition negate_contradict (i1 i2 : nat) (h : hyps) :=
 
 Definition negate_contradict_inv (t i1 i2 : nat) (h : hyps) :=
   match nth_hyps i1 h with
-  | EqTerm (Tint Z0) b1 =>
+  | EqTerm (Tint Nul) b1 =>
       match nth_hyps i2 h with
-      | NeqTerm (Tint Z0) b2 =>
-          match eq_term b1 (scalar_norm t (b2 * Tint (-1))%term) with
-          | true => absurd
-          | false => h
-          end
+      | NeqTerm (Tint Nul') b2 =>
+          if beq Nul 0 && beq Nul' 0 && 
+             eq_term b1 (scalar_norm t (b2 * Tint (-(1)))%term)
+          then absurd
+          else h
       | _ => h
       end
-  | NeqTerm (Tint Z0) b1 =>
+  | NeqTerm (Tint Nul) b1 =>
       match nth_hyps i2 h with
-      | EqTerm (Tint Z0) b2 =>
-          match eq_term b1 (scalar_norm t (b2 * Tint (-1))%term) with
-          | true => absurd
-          | false => h
-          end
+      | EqTerm (Tint Nul') b2 =>
+          if beq Nul 0 && beq Nul' 0 && 
+             eq_term b1 (scalar_norm t (b2 * Tint (-(1)))%term)
+          then absurd
+          else h
       | _ => h
       end
   | _ => h
@@ -1689,45 +2250,33 @@ Definition negate_contradict_inv (t i1 i2 : nat) (h : hyps) :=
 
 Theorem negate_contradict_valid :
  forall i j : nat, valid_hyps (negate_contradict i j).
-
-unfold valid_hyps, negate_contradict in |- *; intros i j ep e l H;
+Proof.
+ unfold valid_hyps, negate_contradict in |- *; intros i j ep e l H;
  generalize (nth_valid _ _ i _ H); generalize (nth_valid _ _ j _ H);
  case (nth_hyps i l); auto; intros t1 t2; case t1; 
- auto; intros z; case z; auto; case (nth_hyps j l); 
- auto; intros t3 t4; case t3; auto; intros z'; case z'; 
- auto; simpl in |- *; intros H1 H2;
- [ elim_eq_term t2 t4; intro H3;
-    [ elim H1; elim H3; assumption | assumption ]
- | elim_eq_term t2 t4; intro H3;
-    [ elim H2; rewrite H3; assumption | assumption ] ].
-
+ auto; intros z; auto; case (nth_hyps j l); 
+ auto; intros t3 t4; case t3; auto; intros z'; 
+ auto; simpl in |- *; intros H1 H2; Simplify.
 Qed.
 
 Theorem negate_contradict_inv_valid :
  forall t i j : nat, valid_hyps (negate_contradict_inv t i j).
-
-
-unfold valid_hyps, negate_contradict_inv in |- *; intros t i j ep e l H;
+Proof.
+ unfold valid_hyps, negate_contradict_inv in |- *; intros t i j ep e l H;
  generalize (nth_valid _ _ i _ H); generalize (nth_valid _ _ j _ H);
  case (nth_hyps i l); auto; intros t1 t2; case t1; 
- auto; intros z; case z; auto; case (nth_hyps j l); 
- auto; intros t3 t4; case t3; auto; intros z'; case z'; 
- auto; simpl in |- *; intros H1 H2;
- (pattern (eq_term t2 (scalar_norm t (t4 * Tint (-1))%term)) in |- *;
-   apply bool_ind2; intro Aux;
-   [ generalize (eq_term_true t2 (scalar_norm t (t4 * Tint (-1))%term) Aux);
-      clear Aux
-   | generalize (eq_term_false t2 (scalar_norm t (t4 * Tint (-1))%term) Aux);
-      clear Aux ]);
- [ intro H3; elim H1; generalize H2; rewrite H3;
-    rewrite <- (scalar_norm_stable t e); simpl in |- *;
-    elim (interp_term e t4); simpl in |- *; auto; intros p H4;
-    discriminate H4
- | auto
- | intro H3; elim H2; rewrite H3; elim (scalar_norm_stable t e);
-    simpl in |- *; elim H1; simpl in |- *; trivial
- | auto ].
-
+ auto; intros z; auto; case (nth_hyps j l); 
+ auto; intros t3 t4; case t3; auto; intros z'; 
+ auto; simpl in |- *; intros H1 H2; Simplify; 
+ [
+ rewrite <- scalar_norm_stable in H2; simpl in *;
+ elim (mult_integral (interp_term e t4) (-(1))); intuition;
+ elim minus_one_neq_zero; auto
+ | 
+ elim H2; clear H2;
+ rewrite <- scalar_norm_stable; simpl in *;
+ now rewrite <- H1, mult_0_l
+ ].
 Qed.
 
 (* \subsubsection{Tactiques générant une nouvelle équation} *)
@@ -1737,150 +2286,93 @@ Qed.
  preuve un peu compliquée. On utilise quelques lemmes qui sont des 
  généralisations des théorèmes utilisés par OMEGA. *)
 
-Definition sum (k1 k2 : Z) (trace : list t_fusion)
+Definition sum (k1 k2 : int) (trace : list t_fusion)
   (prop1 prop2 : proposition) :=
   match prop1 with
-  | EqTerm (Tint Z0) b1 =>
+  | EqTerm (Tint Null) b1 =>
       match prop2 with
-      | EqTerm (Tint Z0) b2 =>
-          EqTerm (Tint 0) (fusion trace (b1 * Tint k1 + b2 * Tint k2)%term)
-      | LeqTerm (Tint Z0) b2 =>
-          match k2 ?= 0 with
-          | Gt =>
-              LeqTerm (Tint 0)
+      | EqTerm (Tint Null') b2 =>
+          if beq Null 0 && beq Null' 0 
+          then EqTerm (Tint 0) (fusion trace (b1 * Tint k1 + b2 * Tint k2)%term)
+          else TrueTerm
+      | LeqTerm (Tint Null') b2 =>
+          if beq Null 0 && beq Null' 0 && bgt k2 0 
+          then LeqTerm (Tint 0)
                 (fusion trace (b1 * Tint k1 + b2 * Tint k2)%term)
-          | _ => TrueTerm
-          end
+          else TrueTerm
       | _ => TrueTerm
       end
-  | LeqTerm (Tint Z0) b1 =>
-      match k1 ?= 0 with
-      | Gt =>
-          match prop2 with
-          | EqTerm (Tint Z0) b2 =>
+  | LeqTerm (Tint Null) b1 =>
+      if beq Null 0 && bgt k1 0
+      then match prop2 with
+          | EqTerm (Tint Null') b2 =>
+              if beq Null' 0 then 
               LeqTerm (Tint 0)
                 (fusion trace (b1 * Tint k1 + b2 * Tint k2)%term)
-          | LeqTerm (Tint Z0) b2 =>
-              match k2 ?= 0 with
-              | Gt =>
-                  LeqTerm (Tint 0)
+              else TrueTerm  
+          | LeqTerm (Tint Null') b2 =>
+              if beq Null' 0 && bgt k2 0 
+              then LeqTerm (Tint 0)
                     (fusion trace (b1 * Tint k1 + b2 * Tint k2)%term)
-              | _ => TrueTerm
-              end
+              else TrueTerm
           | _ => TrueTerm
           end
-      | _ => TrueTerm
-      end
-  | NeqTerm (Tint Z0) b1 =>
+      else TrueTerm 
+  | NeqTerm (Tint Null) b1 =>
       match prop2 with
-      | EqTerm (Tint Z0) b2 =>
-          match eq_Z k1 0 with
-          | true => TrueTerm
-          | false =>
-              NeqTerm (Tint 0)
-                (fusion trace (b1 * Tint k1 + b2 * Tint k2)%term)
-          end
+      | EqTerm (Tint Null') b2 =>
+          if beq Null 0 && beq Null' 0 && (negb (beq k1 0))
+          then NeqTerm (Tint 0)
+                 (fusion trace (b1 * Tint k1 + b2 * Tint k2)%term)
+          else TrueTerm
       | _ => TrueTerm
       end
   | _ => TrueTerm
   end.
 
-Theorem sum1 : forall a b c d : Z, 0 = a -> 0 = b -> 0 = a * c + b * d.
-
-intros; elim H; elim H0; simpl in |- *; auto.
-Qed.
-  
-Theorem sum2 :
- forall a b c d : Z, 0 <= d -> 0 = a -> 0 <= b -> 0 <= a * c + b * d.
-
-intros; elim H0; simpl in |- *; generalize H H1; case b; case d;
- unfold Zle in |- *; simpl in |- *; auto.  
-Qed.
-
-Theorem sum3 :
- forall a b c d : Z,
- 0 <= c -> 0 <= d -> 0 <= a -> 0 <= b -> 0 <= a * c + b * d.
-
-intros a b c d; case a; case b; case c; case d; unfold Zle in |- *;
- simpl in |- *; auto. 
-Qed.
-
-Theorem sum4 : forall k : Z, (k ?= 0) = Gt -> 0 <= k.
-
-intro; case k; unfold Zle in |- *; simpl in |- *; auto; intros; discriminate.  
-Qed.
-
-Theorem sum5 :
- forall a b c d : Z, c <> 0 -> 0 <> a -> 0 = b -> 0 <> a * c + b * d.
-
-intros a b c d H1 H2 H3; elim H3; simpl in |- *; rewrite Zplus_comm;
- simpl in |- *; generalize H1 H2; case a; case c; simpl in |- *; 
- intros; try discriminate; assumption.
-Qed.
-
 
 Theorem sum_valid :
- forall (k1 k2 : Z) (t : list t_fusion), valid2 (sum k1 k2 t).
-
-unfold valid2 in |- *; intros k1 k2 t ep e p1 p2; unfold sum in |- *;
+ forall (k1 k2 : int) (t : list t_fusion), valid2 (sum k1 k2 t).
+Proof.
+ unfold valid2 in |- *; intros k1 k2 t ep e p1 p2; unfold sum in |- *;
  Simplify; simpl in |- *; auto; try elim (fusion_stable t); 
  simpl in |- *; intros;
  [ apply sum1; assumption
  | apply sum2; try assumption; apply sum4; assumption
- | rewrite Zplus_comm; apply sum2; try assumption; apply sum4; assumption
+ | rewrite plus_comm; apply sum2; try assumption; apply sum4; assumption
  | apply sum3; try assumption; apply sum4; assumption
- | elim_eq_Z k1 0; simpl in |- *; auto; elim (fusion_stable t); simpl in |- *;
-    intros; unfold Zne in |- *; apply sum5; assumption ].
+ | apply sum5; auto ].
 Qed.
 
 (* \paragraph{[O_EXACT_DIVIDE]}
    c'est une oper1 valide mais on préfère une substitution a ce point la *)
 
-Definition exact_divide (k : Z) (body : term) (t : nat)
+Definition exact_divide (k : int) (body : term) (t : nat)
   (prop : proposition) :=
   match prop with
-  | EqTerm (Tint Z0) b =>
-      match eq_term (scalar_norm t (body * Tint k)%term) b with
-      | true =>
-          match eq_Z k 0 with
-          | true => TrueTerm
-          | false => EqTerm (Tint 0) body
-          end
-      | false => TrueTerm
-      end
-  | NeqTerm (Tint Z0) b =>
-      match eq_term (scalar_norm t (body * Tint k)%term) b with
-      | true =>
-          match eq_Z k 0 with
-          | true => FalseTerm
-          | false => NeqTerm (Tint 0) body
-          end
-      | false => TrueTerm
-      end
+  | EqTerm (Tint Null) b =>
+      if beq Null 0 && 
+         eq_term (scalar_norm t (body * Tint k)%term) b && 
+         negb (beq k 0) 
+      then EqTerm (Tint 0) body
+      else TrueTerm
+  | NeqTerm (Tint Null) b =>
+      if beq Null 0 && 
+         eq_term (scalar_norm t (body * Tint k)%term) b &&
+         negb (beq k 0)
+      then NeqTerm (Tint 0) body
+      else TrueTerm
   | _ => TrueTerm
   end.
 
 Theorem exact_divide_valid :
- forall (k : Z) (t : term) (n : nat), valid1 (exact_divide k t n).
-
-
-unfold valid1, exact_divide in |- *; intros k1 k2 t ep e p1; Simplify;
- simpl in |- *; auto; elim_eq_term (scalar_norm t (k2 * Tint k1)%term) t1;
- simpl in |- *; auto; elim_eq_Z k1 0; simpl in |- *; 
- auto; intros H1 H2; elim H2; elim scalar_norm_stable;
- simpl in |- *; 
- [
- generalize H1; case (interp_term e k2); 
- try trivial;
- (case k1; simpl in |- *;
-   [ intros; absurd (0 = 0); assumption
-   | intros p2 p3 H3 H4; discriminate H4
-   | intros p2 p3 H3 H4; discriminate H4 ])
- |
- subst k1; rewrite Zmult_comm; simpl in *; intros; absurd (0=0); trivial
- |
- generalize H1; case (interp_term e k2); 
- try trivial; intros p2 p3 H3 H4; discriminate H4
+ forall (k : int) (t : term) (n : nat), valid1 (exact_divide k t n).
+Proof.
+ unfold valid1, exact_divide in |- *; intros k1 k2 t ep e p1; 
+ Simplify; simpl; auto; subst; 
+ rewrite <- scalar_norm_stable; simpl; intros; 
+ [ destruct (mult_integral _ _ (sym_eq H)); intuition
+ | swap H; rewrite <- H1, mult_0_l; auto
  ].
 Qed.
 
@@ -1889,61 +2381,51 @@ Qed.
   La preuve reprend le schéma de la précédente mais on
   est sur une opération de type valid1 et non sur une opération terminale. *)
 
-Definition divide_and_approx (k1 k2 : Z) (body : term) 
+Definition divide_and_approx (k1 k2 : int) (body : term) 
   (t : nat) (prop : proposition) :=
   match prop with
-  | LeqTerm (Tint Z0) b =>
-      match
-        eq_term (scalar_norm_add t (body * Tint k1 + Tint k2)%term) b
-      with
-      | true =>
-          match k1 ?= 0 with
-          | Gt =>
-              match k1 ?= k2 with
-              | Gt => LeqTerm (Tint 0) body
-              | _ => prop
-              end
-          | _ => prop
-          end
-      | false => prop
-      end
+  | LeqTerm (Tint Null) b =>
+      if beq Null 0 && 
+         eq_term (scalar_norm_add t (body * Tint k1 + Tint k2)%term) b &&
+         bgt k1 0 && 
+         bgt k1 k2 
+      then LeqTerm (Tint 0) body 
+      else prop
   | _ => prop
   end.
 
 Theorem divide_and_approx_valid :
- forall (k1 k2 : Z) (body : term) (t : nat),
+ forall (k1 k2 : int) (body : term) (t : nat),
  valid1 (divide_and_approx k1 k2 body t).
-
-unfold valid1, divide_and_approx in |- *; intros k1 k2 body t ep e p1;
- Simplify;
- elim_eq_term (scalar_norm_add t (body * Tint k1 + Tint k2)%term) t1;
- Simplify; auto; intro E; elim E; simpl in |- *;
- elim (scalar_norm_add_stable t e); simpl in |- *; 
- intro H1; apply Zmult_le_approx with (3 := H1); assumption.
+Proof.
+ unfold valid1, divide_and_approx in |- *; intros k1 k2 body t ep e p1;
+ Simplify; simpl; auto; subst;
+ elim (scalar_norm_add_stable t e); simpl in |- *.
+ intro H2; apply mult_le_approx with (3 := H2); assumption.
 Qed.
 
 (* \paragraph{[MERGE_EQ]} *)
 
 Definition merge_eq (t : nat) (prop1 prop2 : proposition) :=
   match prop1 with
-  | LeqTerm (Tint Z0) b1 =>
+  | LeqTerm (Tint Null) b1 =>
       match prop2 with
-      | LeqTerm (Tint Z0) b2 =>
-          match eq_term b1 (scalar_norm t (b2 * Tint (-1))%term) with
-          | true => EqTerm (Tint 0) b1
-          | false => TrueTerm
-          end
+      | LeqTerm (Tint Null') b2 =>
+          if beq Null 0 && beq Null' 0 &&
+             eq_term b1 (scalar_norm t (b2 * Tint (-(1)))%term) 
+          then EqTerm (Tint 0) b1
+          else TrueTerm
       | _ => TrueTerm
       end
   | _ => TrueTerm
   end.
 
 Theorem merge_eq_valid : forall n : nat, valid2 (merge_eq n).
-
-unfold valid2, merge_eq in |- *; intros n ep e p1 p2; Simplify; simpl in |- *;
+Proof.
+ unfold valid2, merge_eq in |- *; intros n ep e p1 p2; Simplify; simpl in |- *;
  auto; elim (scalar_norm_stable n e); simpl in |- *; 
  intros; symmetry  in |- *; apply OMEGA8 with (2 := H0);
- [ assumption | elim Zopp_eq_mult_neg_1; trivial ].
+ [ assumption | elim opp_eq_mult_neg_1; trivial ].
 Qed.
 
 
@@ -1952,36 +2434,39 @@ Qed.
 
 Definition constant_nul (i : nat) (h : hyps) :=
   match nth_hyps i h with
-  | NeqTerm (Tint Z0) (Tint Z0) => absurd
+  | NeqTerm (Tint Null) (Tint Null') => 
+      if beq Null Null' then absurd else h 
   | _ => h
   end.
 
 Theorem constant_nul_valid : forall i : nat, valid_hyps (constant_nul i).
-
-unfold valid_hyps, constant_nul in |- *; intros;
+Proof.
+ unfold valid_hyps, constant_nul in |- *; intros;
  generalize (nth_valid ep e i lp); Simplify; simpl in |- *;
- unfold Zne in |- *; intro H1; absurd (0 = 0); auto.
+ intro H1; absurd (0 = 0); intuition.
 Qed.
 
 (* \paragraph{[O_STATE]} *)
 
-Definition state (m : Z) (s : step) (prop1 prop2 : proposition) :=
+Definition state (m : int) (s : step) (prop1 prop2 : proposition) :=
   match prop1 with
-  | EqTerm (Tint Z0) b1 =>
+  | EqTerm (Tint Null) b1 =>
       match prop2 with
       | EqTerm b2 b3 =>
-          EqTerm (Tint 0) (rewrite s (b1 + (- b3 + b2) * Tint m)%term)
+          if beq Null 0 
+          then EqTerm (Tint 0) (rewrite s (b1 + (- b3 + b2) * Tint m)%term)
+          else TrueTerm
       | _ => TrueTerm
       end
   | _ => TrueTerm
   end.
 
-Theorem state_valid : forall (m : Z) (s : step), valid2 (state m s).
-
-unfold valid2 in |- *; intros m s ep e p1 p2; unfold state in |- *; Simplify;
+Theorem state_valid : forall (m : int) (s : step), valid2 (state m s).
+Proof.
+ unfold valid2 in |- *; intros m s ep e p1 p2; unfold state in |- *; Simplify;
  simpl in |- *; auto; elim (rewrite_stable s e); simpl in |- *; 
  intros H1 H2; elim H1.
- rewrite H2; rewrite Zplus_opp_l; simpl; reflexivity.
+ now rewrite H2, plus_opp_l, plus_0_l, mult_0_l.
 Qed.
 
 (* \subsubsection{Tactiques générant plusieurs but}
@@ -1991,11 +2476,13 @@ Qed.
 Definition split_ineq (i t : nat) (f1 f2 : hyps -> lhyps) 
   (l : hyps) :=
   match nth_hyps i l with
-  | NeqTerm (Tint Z0) b1 =>
-      f1 (LeqTerm (Tint 0) (add_norm t (b1 + Tint (-1))%term) :: l) ++
+  | NeqTerm (Tint Null) b1 =>
+      if beq Null 0 then 
+      f1 (LeqTerm (Tint 0) (add_norm t (b1 + Tint (-(1)))%term) :: l) ++
       f2
         (LeqTerm (Tint 0)
-           (scalar_norm_add t (b1 * Tint (-1) + Tint (-1))%term) :: l)
+           (scalar_norm_add t (b1 * Tint (-(1)) + Tint (-(1)))%term) :: l)
+       else l :: nil
   | _ => l :: nil
   end.
 
@@ -2003,17 +2490,18 @@ Theorem split_ineq_valid :
  forall (i t : nat) (f1 f2 : hyps -> lhyps),
  valid_list_hyps f1 ->
  valid_list_hyps f2 -> valid_list_hyps (split_ineq i t f1 f2).
-
-unfold valid_list_hyps, split_ineq in |- *; intros i t f1 f2 H1 H2 ep e lp H;
+Proof.
+ unfold valid_list_hyps, split_ineq in |- *; intros i t f1 f2 H1 H2 ep e lp H;
  generalize (nth_valid _ _ i _ H); case (nth_hyps i lp); 
  simpl in |- *; auto; intros t1 t2; case t1; simpl in |- *; 
- auto; intros z; case z; simpl in |- *; auto; intro H3; 
+ auto; intros z; simpl in |- *; auto; intro H3.
+ Simplify.
  apply append_valid; elim (OMEGA19 (interp_term e t2));
  [ intro H4; left; apply H1; simpl in |- *; elim (add_norm_stable t);
     simpl in |- *; auto
  | intro H4; right; apply H2; simpl in |- *; elim (scalar_norm_add_stable t);
     simpl in |- *; auto
- | generalize H3; unfold Zne, not in |- *; intros E1 E2; apply E1;
+ | generalize H3; unfold not in |- *; intros E1 E2; apply E1;
     symmetry  in |- *; trivial ].
 Qed.
 
@@ -2046,8 +2534,8 @@ Fixpoint execute_omega (t : t_omega) (l : hyps) {struct t} : lhyps :=
   end.
 
 Theorem omega_valid : forall t : t_omega, valid_list_hyps (execute_omega t).
-
-simple induction t; simpl in |- *;
+Proof.
+ simple induction t; simpl in |- *;
  [ unfold valid_list_hyps in |- *; simpl in |- *; intros; left;
     apply (constant_not_nul_valid n ep e lp H)
  | unfold valid_list_hyps in |- *; simpl in |- *; intros; left;
@@ -2058,7 +2546,7 @@ simple induction t; simpl in |- *;
      (apply_oper_1_valid m (divide_and_approx k1 k2 body n)
         (divide_and_approx_valid k1 k2 body n) ep e lp H)
  | unfold valid_list_hyps in |- *; simpl in |- *; intros; left;
-    apply (not_exact_divide_valid z z0 t0 n n0 ep e lp H)
+    apply (not_exact_divide_valid i i0 t0 n n0 ep e lp H)
  | unfold valid_list_hyps, valid_hyps in |- *;
     intros k body n t' Ht' m ep e lp H; apply Ht';
     apply
@@ -2101,36 +2589,30 @@ Definition move_right (s : step) (p : proposition) :=
   | EqTerm t1 t2 => EqTerm (Tint 0) (rewrite s (t1 + - t2)%term)
   | LeqTerm t1 t2 => LeqTerm (Tint 0) (rewrite s (t2 + - t1)%term)
   | GeqTerm t1 t2 => LeqTerm (Tint 0) (rewrite s (t1 + - t2)%term)
-  | LtTerm t1 t2 => LeqTerm (Tint 0) (rewrite s (t2 + Tint (-1) + - t1)%term)
-  | GtTerm t1 t2 => LeqTerm (Tint 0) (rewrite s (t1 + Tint (-1) + - t2)%term)
+  | LtTerm t1 t2 => LeqTerm (Tint 0) (rewrite s (t2 + Tint (-(1)) + - t1)%term)
+  | GtTerm t1 t2 => LeqTerm (Tint 0) (rewrite s (t1 + Tint (-(1)) + - t2)%term)
   | NeqTerm t1 t2 => NeqTerm (Tint 0) (rewrite s (t1 + - t2)%term)
   | p => p
   end.
 
-Theorem Zne_left_2 : forall x y : Z, Zne x y -> Zne 0 (x + - y).
-unfold Zne, not in |- *; intros x y H1 H2; apply H1;
- apply (Zplus_reg_l (- y)); rewrite Zplus_comm; elim H2; 
- rewrite Zplus_opp_l; trivial.
-Qed.
-
 Theorem move_right_valid : forall s : step, valid1 (move_right s).
-
-unfold valid1, move_right in |- *; intros s ep e p; Simplify; simpl in |- *;
+Proof.
+ unfold valid1, move_right in |- *; intros s ep e p; Simplify; simpl in |- *;
  elim (rewrite_stable s e); simpl in |- *;
- [ symmetry  in |- *; apply Zegal_left; assumption
- | intro; apply Zle_left; assumption
- | intro; apply Zge_left; assumption
- | intro; apply Zgt_left; assumption
- | intro; apply Zlt_left; assumption
- | intro; apply Zne_left_2; assumption ].
+ [ symmetry  in |- *; apply egal_left; assumption
+ | intro; apply le_left; assumption
+ | intro; apply le_left; rewrite <- ge_le_iff; assumption
+ | intro; apply lt_left; rewrite <- gt_lt_iff; assumption
+ | intro; apply lt_left; assumption
+ | intro; apply ne_left_2; assumption ].
 Qed.
 
 Definition do_normalize (i : nat) (s : step) := apply_oper_1 i (move_right s).
 
 Theorem do_normalize_valid :
  forall (i : nat) (s : step), valid_hyps (do_normalize i s).
-
-intros; unfold do_normalize in |- *; apply apply_oper_1_valid;
+Proof.
+ intros; unfold do_normalize in |- *; apply apply_oper_1_valid;
  apply move_right_valid.
 Qed.
 
@@ -2143,42 +2625,39 @@ Fixpoint do_normalize_list (l : list step) (i : nat)
 
 Theorem do_normalize_list_valid :
  forall (l : list step) (i : nat), valid_hyps (do_normalize_list l i).
-
-simple induction l; simpl in |- *; unfold valid_hyps in |- *;
+Proof.
+ simple induction l; simpl in |- *; unfold valid_hyps in |- *;
  [ auto
  | intros a l' Hl' i ep e lp H; unfold valid_hyps in Hl'; apply Hl';
     apply (do_normalize_valid i a ep e lp); assumption ].
 Qed.
 
 Theorem normalize_goal :
- forall (s : list step) (ep : PropList) (env : list Z) (l : hyps),
+ forall (s : list step) (ep : list Prop) (env : list int) (l : hyps),
  interp_goal ep env (do_normalize_list s 0 l) -> interp_goal ep env l.
-
-intros; apply valid_goal with (2 := H); apply do_normalize_list_valid.
+Proof.
+ intros; apply valid_goal with (2 := H); apply do_normalize_list_valid.
 Qed.
 
 (* \subsubsection{Exécution de la trace} *)
 
 Theorem execute_goal :
- forall (t : t_omega) (ep : PropList) (env : list Z) (l : hyps),
+ forall (t : t_omega) (ep : list Prop) (env : list int) (l : hyps),
  interp_list_goal ep env (execute_omega t l) -> interp_goal ep env l.
-
-intros; apply (goal_valid (execute_omega t) (omega_valid t) ep env l H).
+Proof.
+ intros; apply (goal_valid (execute_omega t) (omega_valid t) ep env l H).
 Qed.
 
 
 Theorem append_goal :
- forall (ep : PropList) (e : list Z) (l1 l2 : lhyps),
+ forall (ep : list Prop) (e : list int) (l1 l2 : lhyps),
  interp_list_goal ep e l1 /\ interp_list_goal ep e l2 ->
  interp_list_goal ep e (l1 ++ l2).
-
-intros ep e; simple induction l1;
+Proof.
+ intros ep e; simple induction l1;
  [ simpl in |- *; intros l2 (H1, H2); assumption
  | simpl in |- *; intros h1 t1 HR l2 ((H1, H2), H3); split; auto ].
-
 Qed.
-
-Require Import Decidable.
 
 (* A simple decidability checker : if the proposition belongs to the
    simple grammar describe below then it is decidable. Proof is by 
@@ -2203,30 +2682,29 @@ Fixpoint decidability (p : proposition) : bool :=
   end.
 
 Theorem decidable_correct :
- forall (ep : PropList) (e : list Z) (p : proposition),
+ forall (ep : list Prop) (e : list int) (p : proposition),
  decidability p = true -> decidable (interp_proposition ep e p).
-
-simple induction p; simpl in |- *; intros;
+Proof.
+ simple induction p; simpl in |- *; intros;
  [ apply dec_eq
- | apply dec_Zle
+ | apply dec_le
  | left; auto
  | right; unfold not in |- *; auto
  | apply dec_not; auto
- | apply dec_Zge
- | apply dec_Zgt
- | apply dec_Zlt
- | apply dec_Zne
+ | apply dec_ge
+ | apply dec_gt
+ | apply dec_lt
+ | apply dec_ne
  | apply dec_or; elim andb_prop with (1 := H1); auto
  | apply dec_and; elim andb_prop with (1 := H1); auto
  | apply dec_imp; elim andb_prop with (1 := H1); auto
  | discriminate H ].
-
 Qed.
 
 (* An interpretation function for a complete goal with an explicit
    conclusion. We use an intermediate fixpoint. *)
 
-Fixpoint interp_full_goal (envp : PropList) (env : list Z) 
+Fixpoint interp_full_goal (envp : list Prop) (env : list int) 
  (c : proposition) (l : hyps) {struct l} : Prop :=
   match l with
   | nil => interp_proposition envp env c
@@ -2234,7 +2712,7 @@ Fixpoint interp_full_goal (envp : PropList) (env : list Z)
       interp_proposition envp env p' -> interp_full_goal envp env c l'
   end.
 
-Definition interp_full (ep : PropList) (e : list Z) 
+Definition interp_full (ep : list Prop) (e : list int) 
   (lc : hyps * proposition) : Prop :=
   match lc with
   | (l, c) => interp_full_goal ep e c l
@@ -2244,12 +2722,11 @@ Definition interp_full (ep : PropList) (e : list Z)
    of its hypothesis and conclusion *)
 
 Theorem interp_full_false :
- forall (ep : PropList) (e : list Z) (l : hyps) (c : proposition),
+ forall (ep : list Prop) (e : list int) (l : hyps) (c : proposition),
  (interp_hyps ep e l -> interp_proposition ep e c) -> interp_full ep e (l, c).
-
-simple induction l; unfold interp_full in |- *; simpl in |- *;
+Proof.
+ simple induction l; unfold interp_full in |- *; simpl in |- *;
  [ auto | intros a l1 H1 c H2 H3; apply H1; auto ].
-
 Qed.
 
 (* Push the conclusion in the list of hypothesis using a double negation
@@ -2265,11 +2742,11 @@ Definition to_contradict (lc : hyps * proposition) :=
    hypothesis implies the original goal *)
 
 Theorem to_contradict_valid :
- forall (ep : PropList) (e : list Z) (lc : hyps * proposition),
+ forall (ep : list Prop) (e : list int) (lc : hyps * proposition),
  interp_goal ep e (to_contradict lc) -> interp_full ep e lc.
-
-intros ep e lc; case lc; intros l c; simpl in |- *;
- pattern (decidability c) in |- *; apply bool_ind2;
+Proof.
+ intros ep e lc; case lc; intros l c; simpl in |- *;
+ pattern (decidability c) in |- *; apply bool_eq_ind;
  [ simpl in |- *; intros H H1; apply interp_full_false; intros H2;
     apply not_not;
     [ apply decidable_correct; assumption
@@ -2333,19 +2810,19 @@ Fixpoint destructure_hyps (nn : nat) (ll : hyps) {struct nn} : lhyps :=
   end.
 
 Theorem map_cons_val :
- forall (ep : PropList) (e : list Z) (p : proposition) (l : lhyps),
+ forall (ep : list Prop) (e : list int) (p : proposition) (l : lhyps),
  interp_proposition ep e p ->
  interp_list_hyps ep e l -> interp_list_hyps ep e (map_cons _ p l).
-
-simple induction l; simpl in |- *; [ auto | intros; elim H1; intro H2; auto ].
+Proof.
+ simple induction l; simpl in |- *; [ auto | intros; elim H1; intro H2; auto ].
 Qed.
 
 Hint Resolve map_cons_val append_valid decidable_correct.
 
 Theorem destructure_hyps_valid :
  forall n : nat, valid_list_hyps (destructure_hyps n).
-
-simple induction n;
+Proof.
+ simple induction n;
  [ unfold valid_list_hyps in |- *; simpl in |- *; auto
  | unfold valid_list_hyps at 2 in |- *; intros n1 H ep e lp; case lp;
     [ simpl in |- *; auto
@@ -2358,7 +2835,7 @@ simple induction n;
            (simpl in |- *; intros; apply map_cons_val; simpl in |- *; elim H0;
              auto);
           [ simpl in |- *; intros p1 (H1, H2);
-             pattern (decidability p1) in |- *; apply bool_ind2; 
+             pattern (decidability p1) in |- *; apply bool_eq_ind; 
              intro H3;
              [ apply H; simpl in |- *; split;
                 [ apply not_not; auto | assumption ]
@@ -2366,7 +2843,7 @@ simple induction n;
           | simpl in |- *; intros p1 p2 (H1, H2); apply H; simpl in |- *;
              elim not_or with (1 := H1); auto
           | simpl in |- *; intros p1 p2 (H1, H2);
-             pattern (decidability p1) in |- *; apply bool_ind2; 
+             pattern (decidability p1) in |- *; apply bool_eq_ind; 
              intro H3;
              [ apply append_valid; elim not_and with (2 := H1);
                 [ intro; left; apply H; simpl in |- *; auto
@@ -2378,18 +2855,17 @@ simple induction n;
           apply H; simpl in |- *; auto
        | simpl in |- *; intros; apply H; simpl in |- *; tauto
        | simpl in |- *; intros p1 p2 (H1, H2);
-          pattern (decidability p1) in |- *; apply bool_ind2; 
+          pattern (decidability p1) in |- *; apply bool_eq_ind; 
           intro H3;
           [ apply append_valid; elim imp_simp with (2 := H1);
              [ intro H4; left; simpl in |- *; apply H; simpl in |- *; auto
              | intro H4; right; simpl in |- *; apply H; simpl in |- *; auto
              | auto ]
           | auto ] ] ] ].
-
 Qed.
 
 Definition prop_stable (f : proposition -> proposition) :=
-  forall (ep : PropList) (e : list Z) (p : proposition),
+  forall (ep : list Prop) (e : list int) (p : proposition),
   interp_proposition ep e p <-> interp_proposition ep e (f p).
 
 Definition p_apply_left (f : proposition -> proposition) 
@@ -2405,8 +2881,8 @@ Definition p_apply_left (f : proposition -> proposition)
 Theorem p_apply_left_stable :
  forall f : proposition -> proposition,
  prop_stable f -> prop_stable (p_apply_left f).
-
-unfold prop_stable in |- *; intros f H ep e p; split;
+Proof.
+ unfold prop_stable in |- *; intros f H ep e p; split;
  (case p; simpl in |- *; auto; intros p1; elim (H ep e p1); tauto).
 Qed.
 
@@ -2423,8 +2899,8 @@ Definition p_apply_right (f : proposition -> proposition)
 Theorem p_apply_right_stable :
  forall f : proposition -> proposition,
  prop_stable f -> prop_stable (p_apply_right f).
-
-unfold prop_stable in |- *; intros f H ep e p; split;
+Proof.
+ unfold prop_stable in |- *; intros f H ep e p; split;
  (case p; simpl in |- *; auto;
    [ intros p1; elim (H ep e p1); tauto
    | intros p1 p2; elim (H ep e p2); tauto
@@ -2447,67 +2923,55 @@ Definition p_invert (f : proposition -> proposition)
 Theorem p_invert_stable :
  forall f : proposition -> proposition,
  prop_stable f -> prop_stable (p_invert f).
-
-unfold prop_stable in |- *; intros f H ep e p; split;
+Proof.
+ unfold prop_stable in |- *; intros f H ep e p; split;
  (case p; simpl in |- *; auto;
    [ intros t1 t2; elim (H ep e (NeqTerm t1 t2)); simpl in |- *;
-      unfold Zne in |- *;
       generalize (dec_eq (interp_term e t1) (interp_term e t2));
       unfold decidable in |- *; tauto
    | intros t1 t2; elim (H ep e (GtTerm t1 t2)); simpl in |- *;
-      unfold Zgt in |- *;
-      generalize (dec_Zgt (interp_term e t1) (interp_term e t2));
-      unfold decidable, Zgt, Zle in |- *; tauto
+      generalize (dec_gt (interp_term e t1) (interp_term e t2));
+      unfold decidable in |- *; rewrite le_lt_iff, <- gt_lt_iff; tauto
    | intros t1 t2; elim (H ep e (LtTerm t1 t2)); simpl in |- *;
-      unfold Zlt in |- *;
-      generalize (dec_Zlt (interp_term e t1) (interp_term e t2));
-      unfold decidable, Zge in |- *; tauto
+      generalize (dec_lt (interp_term e t1) (interp_term e t2));
+      unfold decidable in |- *; rewrite ge_le_iff, le_lt_iff; tauto
    | intros t1 t2; elim (H ep e (LeqTerm t1 t2)); simpl in |- *;
-      generalize (dec_Zgt (interp_term e t1) (interp_term e t2));
-      unfold Zle, Zgt in |- *; unfold decidable in |- *; 
-      tauto
+      generalize (dec_gt (interp_term e t1) (interp_term e t2));
+      unfold decidable in |- *; repeat rewrite le_lt_iff;
+      repeat rewrite gt_lt_iff; tauto
    | intros t1 t2; elim (H ep e (GeqTerm t1 t2)); simpl in |- *;
-      generalize (dec_Zlt (interp_term e t1) (interp_term e t2));
-      unfold Zge, Zlt in |- *; unfold decidable in |- *; 
-      tauto
+      generalize (dec_lt (interp_term e t1) (interp_term e t2));
+      unfold decidable in |- *; repeat rewrite ge_le_iff;
+      repeat rewrite le_lt_iff; tauto
    | intros t1 t2; elim (H ep e (EqTerm t1 t2)); simpl in |- *;
       generalize (dec_eq (interp_term e t1) (interp_term e t2));
-      unfold decidable, Zne in |- *; tauto ]).
-Qed.
-
-Theorem Zlt_left_inv : forall x y : Z, 0 <= y + -1 + - x -> x < y.
-
-intros; apply Zsucc_lt_reg; apply Zle_lt_succ;
- apply (fun a b : Z => Zplus_le_reg_r a b (-1 + - x)); 
- rewrite Zplus_assoc; unfold Zsucc in |- *; rewrite (Zplus_assoc_reverse x);
- rewrite (Zplus_assoc y); simpl in |- *; rewrite Zplus_0_r;
- rewrite Zplus_opp_r; assumption.
+      unfold decidable; tauto ]).
 Qed.
 
 Theorem move_right_stable : forall s : step, prop_stable (move_right s).
-
-unfold move_right, prop_stable in |- *; intros s ep e p; split;
+Proof.
+ unfold move_right, prop_stable in |- *; intros s ep e p; split;
  [ Simplify; simpl in |- *; elim (rewrite_stable s e); simpl in |- *;
-    [ symmetry  in |- *; apply Zegal_left; assumption
-    | intro; apply Zle_left; assumption
-    | intro; apply Zge_left; assumption
-    | intro; apply Zgt_left; assumption
-    | intro; apply Zlt_left; assumption
-    | intro; apply Zne_left_2; assumption ]
+    [ symmetry  in |- *; apply egal_left; assumption
+    | intro; apply le_left; assumption
+    | intro; apply le_left; rewrite <- ge_le_iff; assumption
+    | intro; apply lt_left; rewrite <- gt_lt_iff; assumption
+    | intro; apply lt_left; assumption
+    | intro; apply ne_left_2; assumption ]
  | case p; simpl in |- *; intros; auto; generalize H; elim (rewrite_stable s);
     simpl in |- *; intro H1;
-    [ rewrite (Zplus_0_r_reverse (interp_term e t0)); rewrite H1;
-       rewrite Zplus_permute; rewrite Zplus_opp_r; 
-       rewrite Zplus_0_r; trivial
-    | apply (fun a b : Z => Zplus_le_reg_r a b (- interp_term e t));
-       rewrite Zplus_opp_r; assumption
-    | apply Zle_ge;
-       apply (fun a b : Z => Zplus_le_reg_r a b (- interp_term e t0));
-       rewrite Zplus_opp_r; assumption
-    | apply Zlt_gt; apply Zlt_left_inv; assumption
-    | apply Zlt_left_inv; assumption
-    | unfold Zne, not in |- *; unfold Zne in H1; intro H2; apply H1;
-       rewrite H2; rewrite Zplus_opp_r; trivial ] ].
+    [ rewrite (plus_0_r_reverse (interp_term e t0)); rewrite H1;
+       rewrite plus_permute; rewrite plus_opp_r; 
+       rewrite plus_0_r; trivial
+    | apply (fun a b => plus_le_reg_r a b (- interp_term e t));
+       rewrite plus_opp_r; assumption
+    | rewrite ge_le_iff;
+       apply (fun a b => plus_le_reg_r a b (- interp_term e t0));
+       rewrite plus_opp_r; assumption
+    | rewrite gt_lt_iff; apply lt_left_inv; assumption
+    | apply lt_left_inv; assumption
+    | unfold not in |- *; intro H2; apply H1;
+       rewrite H2; rewrite plus_opp_r; trivial ] ].
 Qed.
 
 
@@ -2521,9 +2985,8 @@ Fixpoint p_rewrite (s : p_step) : proposition -> proposition :=
   end.
 
 Theorem p_rewrite_stable : forall s : p_step, prop_stable (p_rewrite s).
-
-
-simple induction s; simpl in |- *;
+Proof.
+ simple induction s; simpl in |- *;
  [ intros; apply p_apply_left_stable; trivial
  | intros; apply p_apply_right_stable; trivial
  | intros; apply p_invert_stable; apply move_right_stable
@@ -2539,8 +3002,8 @@ Fixpoint normalize_hyps (l : list h_step) (lh : hyps) {struct l} : hyps :=
 
 Theorem normalize_hyps_valid :
  forall l : list h_step, valid_hyps (normalize_hyps l).
-
-simple induction l; unfold valid_hyps in |- *; simpl in |- *;
+Proof.
+ simple induction l; unfold valid_hyps in |- *; simpl in |- *;
  [ auto
  | intros n_s r; case n_s; intros n s H ep e lp H1; apply H;
     apply apply_oper_1_valid;
@@ -2550,10 +3013,10 @@ simple induction l; unfold valid_hyps in |- *; simpl in |- *;
 Qed.
 
 Theorem normalize_hyps_goal :
- forall (s : list h_step) (ep : PropList) (env : list Z) (l : hyps),
+ forall (s : list h_step) (ep : list Prop) (env : list int) (l : hyps),
  interp_goal ep env (normalize_hyps s l) -> interp_goal ep env l.
-
-intros; apply valid_goal with (2 := H); apply normalize_hyps_valid.
+Proof.
+ intros; apply valid_goal with (2 := H); apply normalize_hyps_valid.
 Qed.
 
 Fixpoint extract_hyp_pos (s : list direction) (p : proposition) {struct s} :
@@ -2604,18 +3067,18 @@ Fixpoint extract_hyp_pos (s : list direction) (p : proposition) {struct s} :
   end.
 
 Definition co_valid1 (f : proposition -> proposition) :=
-  forall (ep : PropList) (e : list Z) (p1 : proposition),
+  forall (ep : list Prop) (e : list int) (p1 : proposition),
   interp_proposition ep e (Tnot p1) -> interp_proposition ep e (f p1).
 
 Theorem extract_valid :
  forall s : list direction,
  valid1 (extract_hyp_pos s) /\ co_valid1 (extract_hyp_neg s).
-
-unfold valid1, co_valid1 in |- *; simple induction s;
+Proof.
+ unfold valid1, co_valid1 in |- *; simple induction s;
  [ split;
     [ simpl in |- *; auto
     | intros ep e p1; case p1; simpl in |- *; auto; intro p;
-       pattern (decidability p) in |- *; apply bool_ind2;
+       pattern (decidability p) in |- *; apply bool_eq_ind;
        [ intro H; generalize (decidable_correct ep e p H);
           unfold decidable in |- *; tauto
        | simpl in |- *; auto ] ]
@@ -2623,12 +3086,11 @@ unfold valid1, co_valid1 in |- *; simple induction s;
     case p; auto; simpl in |- *; intros;
     (apply H1; tauto) ||
       (apply H2; tauto) ||
-        (pattern (decidability p0) in |- *; apply bool_ind2;
+        (pattern (decidability p0) in |- *; apply bool_eq_ind;
           [ intro H3; generalize (decidable_correct ep e p0 H3);
              unfold decidable in |- *; intro H4; apply H1; 
              tauto
           | intro; tauto ]) ].
-
 Qed.
 
 Fixpoint decompose_solve (s : e_step) (h : hyps) {struct s} : lhyps :=
@@ -2655,13 +3117,13 @@ Fixpoint decompose_solve (s : e_step) (h : hyps) {struct s} : lhyps :=
 
 Theorem decompose_solve_valid :
  forall s : e_step, valid_list_goal (decompose_solve s).
-
-intro s; apply goal_valid; unfold valid_list_hyps in |- *; elim s;
+Proof.
+ intro s; apply goal_valid; unfold valid_list_hyps in |- *; elim s;
  simpl in |- *; intros;
  [ cut (interp_proposition ep e1 (extract_hyp_pos l (nth_hyps n lp)));
     [ case (extract_hyp_pos l (nth_hyps n lp)); simpl in |- *; auto;
        [ intro p; case p; simpl in |- *; auto; intros p1 p2 H2;
-          pattern (decidability p1) in |- *; apply bool_ind2;
+          pattern (decidability p1) in |- *; apply bool_eq_ind;
           [ intro H3; generalize (decidable_correct ep e1 p1 H3); intro H4;
              apply append_valid; elim H4; intro H5;
              [ right; apply H0; simpl in |- *; tauto
@@ -2671,7 +3133,7 @@ intro s; apply goal_valid; unfold valid_list_hyps in |- *; elim s;
           [ intros H3; left; apply H; simpl in |- *; auto
           | intros H3; right; apply H0; simpl in |- *; auto ] 
        | intros p1 p2 H2;
-         pattern (decidability p1) in |- *; apply bool_ind2;
+         pattern (decidability p1) in |- *; apply bool_eq_ind;
           [ intro H3; generalize (decidable_correct ep e1 p1 H3); intro H4;
              apply append_valid; elim H4; intro H5; 
              [ right; apply H0; simpl in |- *; tauto
@@ -2687,7 +3149,7 @@ Qed.
 (* \subsection{La dernière étape qui élimine tous les séquents inutiles} *)
 
 Definition valid_lhyps (f : lhyps -> lhyps) :=
-  forall (ep : PropList) (e : list Z) (lp : lhyps),
+  forall (ep : list Prop) (e : list int) (lp : lhyps),
   interp_list_hyps ep e lp -> interp_list_hyps ep e (f lp).
 
 Fixpoint reduce_lhyps (lp : lhyps) : lhyps :=
@@ -2698,8 +3160,8 @@ Fixpoint reduce_lhyps (lp : lhyps) : lhyps :=
   end.
 
 Theorem reduce_lhyps_valid : valid_lhyps reduce_lhyps.
-
-unfold valid_lhyps in |- *; intros ep e lp; elim lp;
+Proof.
+ unfold valid_lhyps in |- *; intros ep e lp; elim lp;
  [ simpl in |- *; auto
  | intros a l HR; elim a;
     [ simpl in |- *; tauto
@@ -2707,10 +3169,10 @@ unfold valid_lhyps in |- *; intros ep e lp; elim lp;
 Qed.
 
 Theorem do_reduce_lhyps :
- forall (envp : PropList) (env : list Z) (l : lhyps),
+ forall (envp : list Prop) (env : list int) (l : lhyps),
  interp_list_goal envp env (reduce_lhyps l) -> interp_list_goal envp env l.
-
-intros envp env l H; apply list_goal_to_hyps; intro H1;
+Proof.
+ intros envp env l H; apply list_goal_to_hyps; intro H1;
  apply list_hyps_to_goal with (1 := H); apply reduce_lhyps_valid; 
  assumption.
 Qed.
@@ -2719,13 +3181,13 @@ Definition concl_to_hyp (p : proposition) :=
   if decidability p then Tnot p else TrueTerm.
 
 Definition do_concl_to_hyp :
-  forall (envp : PropList) (env : list Z) (c : proposition) (l : hyps),
+  forall (envp : list Prop) (env : list int) (c : proposition) (l : hyps),
   interp_goal envp env (concl_to_hyp c :: l) ->
   interp_goal_concl c envp env l.
-
-simpl in |- *; intros envp env c l; induction l as [| a l Hrecl];
+Proof.
+ simpl in |- *; intros envp env c l; induction l as [| a l Hrecl];
  [ simpl in |- *; unfold concl_to_hyp in |- *;
-    pattern (decidability c) in |- *; apply bool_ind2;
+    pattern (decidability c) in |- *; apply bool_eq_ind;
     [ intro H; generalize (decidable_correct envp env c H);
        unfold decidable in |- *; simpl in |- *; tauto
     | simpl in |- *; intros H1 H2; elim H2; trivial ]
@@ -2737,12 +3199,19 @@ Definition omega_tactic (t1 : e_step) (t2 : list h_step)
   reduce_lhyps (decompose_solve t1 (normalize_hyps t2 (concl_to_hyp c :: l))).
 
 Theorem do_omega :
- forall (t1 : e_step) (t2 : list h_step) (envp : PropList) 
-   (env : list Z) (c : proposition) (l : hyps),
+ forall (t1 : e_step) (t2 : list h_step) (envp : list Prop) 
+   (env : list int) (c : proposition) (l : hyps),
  interp_list_goal envp env (omega_tactic t1 t2 c l) ->
  interp_goal_concl c envp env l.
-
-unfold omega_tactic in |- *; intros; apply do_concl_to_hyp;
+Proof.
+ unfold omega_tactic in |- *; intros; apply do_concl_to_hyp;
  apply (normalize_hyps_goal t2); apply (decompose_solve_valid t1);
  apply do_reduce_lhyps; assumption.
 Qed.
+
+End IntOmega.
+
+(* For now, the above modular construction is instanciated on Z, 
+   in order to retrieve the initial ROmega. *)
+
+Module ZOmega := IntOmega(Z_as_Int).
